theories/theories/utp_csp.thy
@@ -20,104 +20,27 @@ abbreviation "CSP2 \<equiv> H2"
 definition CSP :: "'a WF_PREDICATE \<Rightarrow> 'a WF_PREDICATE" where
 "CSP P = (CSP1 \<circ> CSP2 \<circ> RH) P"
 
-definition Skip :: "'a WF_PREDICATE" where
-"Skip = `RH(\<exists> ref. II\<^bsub>rea\<^esub>)`"
-
-declare CSP1_def [eval, evalr, evalrr, evalrx]
-declare CSP_def [eval, evalr, evalrr, evalrx]
-declare \<delta>_def [eval, evalr, evalrr, evalrx]
-declare doA_def [eval, evalr, evalrr, evalrx]
-declare \<Phi>_def [eval, evalr, evalrr, evalrx]
-declare B_def [eval, evalr, evalrr, evalrx]
-
-lemma CSP1_idempotent: "`CSP1(CSP1(P))` = `CSP1(P)`" 
-  by (utp_pred_auto_tac)
-
-lemma CSP2_idempotent: "`CSP2(CSP2(P))` = `CSP2(P)`"
-  by (metis H2_idempotent)
-
-lemma CSP1_monotonic: 
-  "P \<sqsubseteq> Q \<Longrightarrow> CSP1(P) \<sqsubseteq> CSP1(Q)"
-  by (utp_pred_tac)
-
-lemma CSP2_monotonic:
-  "P \<sqsubseteq> Q \<Longrightarrow> CSP2(P) \<sqsubseteq> CSP2(Q)"
-  by (metis H2_monotone)
-
-lemma CSP1_CSP2_commute: 
-  assumes "P \<in> WF_RELATION"
-  shows "CSP1 (CSP2 P) = CSP2 (CSP1 P)" 
-  apply (simp add: CSP1_def usubst typing defined closure H2_def SemiR_OrP_distr)
-  apply (metis (hide_lams, no_types) DesignD_extreme_point_nok(2) H1_H2_commute H1_def H2_def R1_H2_commute R1_def SemiR_FalseP_left TopD_rel_closure utp_pred_simps(15))
-done
-  
-lemma CSP1_false_is_CSP2 : "`(\<not> ok \<and> ($tr \<le> $tr\<acute>)) ; J` = `(\<not> ok \<and> ($tr \<le> $tr\<acute>))`" sorry
-lemma \<delta>_and_SKIP_is_false : "`((ok\<acute> \<and> \<delta>) \<and> (\<not> ok \<and> ($tr \<le> $tr\<acute>)) \<and> SKIP) ; J \<or> Q` = `Q`" sorry
-lemma aid : "`((\<not> ok \<and> ($tr \<le> $tr\<acute>)) \<and> (\<not> ok \<and> ($tr \<le> $tr\<acute>)) \<and> SKIP) ; J` =`(\<not> ok \<and> ($tr \<le> $tr\<acute>))`" oops
-lemma CSP2_form: "`CSP2(P)` = `P\<^sup>f \<or> ok'\<and> P\<^sup>t`"sorry
-lemma SkipREA_is_CSP2 : "`CSP2(II\<^bsub>rea\<^esub>)` = `II\<^bsub>rea\<^esub>`"sorry
-lemma R3_form : "`R3(P)` = `II\<^bsub>rea\<^esub> \<lhd> $wait \<rhd> (P\<^sub>f)`"sorry
-
-lemma CSP1_R1_commute: "CSP1 (R1 P) = R1 (CSP1 (P))"by utp_pred_auto_tac
-lemma CSP1_R2_commute: "CSP1 (R2 P) = R2 (CSP1 (P))"by(simp add:CSP1_def R2_def R2s_def usubst typing defined closure, utp_pred_auto_tac)
-lemma CSP1_R3_commute: "CSP1 (R3 P) = R3 (CSP1 (P))"by utp_pred_auto_tac
-lemma CSP2_R1_commute: "CSP2 (R1 P) = R1 (CSP2 (P))"by (simp add:CSP2_form, utp_pred_auto_tac)
-lemma CSP2_R2_commute: "CSP2 (R2 P) = R2 (CSP2 (P))"sorry
-lemma CSP2_R3_commute: "CSP2 (R3 P) = R3 (CSP2 (P))" 
-proof -
-have "CSP2 (R3 P) = `($wait \<and> CSP2(II\<^bsub>rea\<^esub>)) \<or> (\<not> $wait \<and> CSP2(P))`" 
-  apply(simp add:CSP2_form R3_def CondR_def usubst typing defined closure)
-  apply utp_pred_auto_tac
-done
-thus ?thesis by (simp add:SkipREA_is_CSP2 CondR_def R3_def)
-qed
-
-lemma commuting_substitutions : "`R2s(P)[false/wait]` = `R2s(P [false/wait])`" apply(simp add:R2s_def)  sorry
-
-lemma DesignD_form : "`(P \<turnstile> Q)` = `\<not>ok \<or> \<not>P \<or> (ok' \<and> Q)`" by(simp add:DesignD_def, utp_pred_auto_tac)
-
-lemma CSP_Closure : "P is CSP \<longleftrightarrow> `R(\<not> P\<^sup>f\<^sub>f \<turnstile> P\<^sup>t\<^sub>f)` = P"
-  sorry
-
-(*
-proof -
-have "`R(\<not> P\<^sup>f\<^sub>f \<turnstile> P\<^sup>t\<^sub>f)` = `R1(R3( \<not>ok \<or> R2s(P\<^sup>f\<^sub>f) \<or> R2s(ok'\<and>  P\<^sup>t\<^sub>f)))`" apply(simp add:RH_def R2_def R1_idempotent R2_R3_commute DesignD_form R2s_OrP R2s_not_ok)
-also have "... = `R1(($wait \<and> II\<^bsub>rea\<^esub>) \<or> (\<not>$wait \<and> \<not>ok) \<or> (\<not>$wait \<and> R2s(P\<^sup>f\<^sub>f)) \<or> (\<not>$wait\<and> ok'\<and> R2s(P\<^sup>t\<^sub>f)))`" sorry (* apply (simp add:R3_def CondR_def R2s_distributes_through_conjunction ok_dash_is_R2s, utp_pred_auto_tac) *)
-also have "... = `($wait \<and> \<not>ok \<and> ($tr \<le> $tr\<acute>)) \<or> ($wait \<and> ok' \<and> ($tr \<le> $tr\<acute>) \<and> II\<^bsub>REL_VAR - {okay\<down>, okay\<down>\<acute>}\<^esub>) \<or> (\<not>$wait \<and> ($tr \<le> $tr\<acute>) \<and> \<not>ok) \<or> (\<not>$wait \<and> ($tr \<le> $tr\<acute>) \<and> R2s(P\<^sup>f\<^sub>f)) \<or> (\<not>$wait\<and> ok'\<and> ($tr \<le> $tr\<acute>) \<and> R2s(P\<^sup>t\<^sub>f))`" by utp_pred_auto_tac
-also have "... = `(\<not>ok \<and> ($tr \<le> $tr\<acute>)) \<or> ($wait \<and> \<not>ok \<and> ($tr \<le> $tr\<acute>)) \<or> ($wait \<and> ok' \<and> ($tr \<le> $tr\<acute>) \<and> II\<^bsub>REL_VAR - {okay\<down>, okay\<down>\<acute>}\<^esub>) \<or> (\<not>$wait \<and> ($tr \<le> $tr\<acute>) \<and> R2(P\<^sup>f\<^sub>f)) \<or> (\<not>$wait\<and> ok'\<and> ($tr \<le> $tr\<acute>) \<and> R2s(P\<^sup>t\<^sub>f))`" by utp_pred_auto_tac
-also have "... = `CSP1(R1(($wait \<and> ( \<not>ok  \<or> (ok'  \<and> II\<^bsub>REL_VAR - {okay\<down>, okay\<down>\<acute>}\<^esub>))) \<or> (\<not>$wait \<and> (R2s(P\<^sup>f\<^sub>f) \<or> (ok'\<and> R2s(P\<^sup>t\<^sub>f))))))`" by utp_pred_auto_tac
-also have "... = `CSP1(R1(($wait \<and> ( \<not>ok  \<or> (ok'  \<and> II\<^bsub>REL_VAR - {okay\<down>, okay\<down>\<acute>}\<^esub>))) \<or> (\<not>$wait \<and> (R2s(P\<^sup>f) \<or> (ok'\<and> R2s(P\<^sup>t)))\<^sub>f)))`" by(simp add:usubst typing closure defined, simp add:commuting_substitutions)
-also have "... = `CSP1(R1(R3(R2s(P\<^sup>f) \<or> ( ok'\<and> R2s(P\<^sup>t)))))`" by(simp add:R3_form CondR_def SkipREA_def, utp_pred_auto_tac)
-also have "... = `CSP1(R1(R3(R2s(P\<^sup>f \<or> ( ok'\<and> P\<^sup>t)))))`" sorry (* by (simp add:R2s_distributes_through_disjunction R2s_distributes_through_conjunction ok_dash_is_R2s) *)
-also have "... = `CSP1(R1(R2(R3(CSP2(P)))))`" by(simp add:R2_def R1_idempotent R2s_R3_commute CSP2_form)
-also have "... = `CSP(P)`" by (simp add:CSP_def R_def CSP2_R1_commute CSP2_R2_commute CSP2_R3_commute)
-finally show ?thesis by(simp add:is_healthy_def)
-qed
-*)
-
-definition deadlock :: "'a WF_PREDICATE" ("STOP") where
+definition StopCSP :: "'a WF_PREDICATE" ("STOP") where
 "STOP = `CSP1( ok' \<and> \<delta>)`"
 
-definition prefix :: "('m EVENT, 'm) WF_PEXPRESSION \<Rightarrow> 'm WF_PREDICATE" ("_ \<rightarrow> SKIP") where
+definition PrefixSkipCSP :: "('m EVENT, 'm) WF_PEXPRESSION \<Rightarrow> 'm WF_PREDICATE" ("_ \<rightarrow> SKIP") where
 "a \<rightarrow> SKIP = `CSP1(ok' \<and> do\<A>(a))`"
 
 definition SkipCSP :: "'a WF_PREDICATE" ("SKIP") where 
-"SKIP = `CSP1(R3(ok' \<and> (\<exists> ref . II\<^bsub>rea\<^esub>)))`"
-
-definition ChaosCSP :: "'a WF_PREDICATE" ("CHAOS") where
-"CHAOS = `CSP1(R1(R3(true)))`"
+"SKIP = `RH(\<exists> ref . II\<^bsub>rea\<^esub>)`"
 
 syntax
-  "_upred_deadlock" :: "upred" ("STOP")
-  "_upred_prefix" :: "uexpr \<Rightarrow> upred" ("@_")
-  "_upred_skip" :: "upred" ("SKIP")
-  "_upred_chaos" :: "upred" ("CHAOS")
+  "_upred_StopCSP" :: "upred" ("STOP")
+  "_upred_PrefixSkipCSP" :: "uexpr \<Rightarrow> upred" ("@_")
+  "_upred_SkipCSP" :: "upred" ("SKIP")
   
 translations
-  "_upred_deadlock" == "CONST deadlock"
-  "_upred_prefix a" == "CONST prefix a"
-  "_upred_skip" == "CONST SkipCSP"
-  "_upred_chaos" == "CONST ChaosCSP"
+  "_upred_StopCSP" == "CONST StopCSP"
+  "_upred_PrefixSkipCSP a" == "CONST PrefixSkipCSP a"
+  "_upred_SkipCSP" == "CONST SkipCSP"
+
+definition ChaosCSP :: "'a WF_PREDICATE" ("CHAOS") where
+"CHAOS = `CSP1(RH(true))`"
 
 definition PrefixCSP :: 
   "('a EVENT, 'a) WF_PEXPRESSION \<Rightarrow> 'a WF_PREDICATE \<Rightarrow> 'a WF_PREDICATE" ("_\<rightarrow>_") where
@@ -130,7 +53,7 @@ definition OutputCSP ::
   "'b::type CHAN \<Rightarrow> ('b, 'a) WF_PEXPRESSION \<Rightarrow> 'a WF_PREDICATE \<Rightarrow> 'a WF_PREDICATE" where
 "OutputCSP n v P = PrefixCSP (EventPE n v) P"
 
-definition ExtChoiceCSP :: 
+definition ExternalChoiceCSP :: 
   "'a WF_PREDICATE \<Rightarrow> 'a WF_PREDICATE \<Rightarrow> 'a WF_PREDICATE" (infixl "\<box>" 65) where
 "P \<box> Q = `CSP2((P \<and> Q)\<lhd> STOP \<rhd>(P \<or> Q))`"
 
@@ -163,7 +86,12 @@ definition ParallelCSP ::
    'a WF_PREDICATE" (infix "\<parallel>\<^bsub>CSP'(_')\<^esub>" 100) where
 "P \<parallel>\<^bsub>CSP(A)\<^esub> Q = P \<parallel>\<^bsub>MergeCSP A\<^esub> Q"
 
+definition InterleaveCSP 
+  :: "'a WF_PREDICATE \<Rightarrow> 'a WF_PREDICATE \<Rightarrow> 'a WF_PREDICATE" (infix "|||\<^bsub>CSP\<^esub>" 100) where
+"P |||\<^bsub>CSP\<^esub> Q = ParallelCSP P |{}| Q"
+
 syntax
+  "_upred_ChaosCSP" :: "upred" ("CHAOS")
   "_upred_prefixed"  :: "pexpr \<Rightarrow> upred \<Rightarrow> upred" ("_ -> _")
   "_upred_input"     :: "'a CHAN \<Rightarrow> pttrn \<Rightarrow> upred \<Rightarrow> upred" ("_?_ -> _")
   "_upred_output"    :: "'a CHAN \<Rightarrow> pexpr \<Rightarrow> upred \<Rightarrow> upred" ("_!_ -> _")
@@ -177,101 +105,820 @@ syntax (xsymbols)
   "_upred_output"    :: "'a CHAN \<Rightarrow> pexpr \<Rightarrow> upred \<Rightarrow> upred" ("_!_ \<rightarrow> _")
   "_upred_extchoice" :: "upred \<Rightarrow> upred \<Rightarrow> upred" (infixl "\<box>" 65)
   "_upred_parallel"  :: "upred \<Rightarrow> pexpr \<Rightarrow> upred \<Rightarrow> upred" (infixr "\<parallel>\<^bsub>_\<^esub>" 100)
+  "_upred_interleave" :: "upred \<Rightarrow> upred \<Rightarrow> upred" (infix "|||" 100)
 
 translations
+  "_upred_ChaosCSP" == "CONST ChaosCSP"
   "_upred_prefixed a P"   == "CONST PrefixCSP a P"
   "_upred_input n v p"    == "CONST InputCSP n (\<lambda> v. p)"
   "_upred_output n v p"   == "CONST OutputCSP n v p"
-  "_upred_extchoice P Q"  == "CONST ExtChoiceCSP P Q"
+  "_upred_extchoice P Q"  == "CONST ExternalChoiceCSP P Q"
   "_upred_guardcsp b P"   == "CONST GuardCSP b P"
   "_upred_parallel P A Q" == "CONST ParallelCSP P A Q"
-
-definition InterleaveCSP 
-  :: "'a WF_PREDICATE \<Rightarrow> 'a WF_PREDICATE \<Rightarrow> 'a WF_PREDICATE" (infix "|||\<^bsub>CSP\<^esub>" 100) where
-"P |||\<^bsub>CSP\<^esub> Q = ParallelCSP P |{}| Q"
-
-syntax
-  "_upred_interleave" :: "upred \<Rightarrow> upred \<Rightarrow> upred" (infix "|||" 100)
- 
-translations
   "_upred_interleave P Q" == "CONST InterleaveCSP P Q"
 
-declare deadlock_def [eval, evalr, evalrr, evalrx]
-declare prefix_def [eval, evalr, evalrr, evalrx]
+declare CSP1_def [eval, evalr, evalrr, evalrx]
+declare CSP_def [eval, evalr, evalrr, evalrx]
+declare StopCSP_def [eval, evalr, evalrr, evalrx]
+declare PrefixSkipCSP_def [eval, evalr, evalrr, evalrx]
 declare SkipCSP_def [eval, evalr, evalrr, evalrx]
 declare ChaosCSP_def [eval, evalr, evalrr, evalrx]
 declare PrefixCSP_def [eval, evalr, evalrr, evalrx]
-declare ExtChoiceCSP_def [eval, evalr, evalrr, evalrx]
+declare ExternalChoiceCSP_def [eval, evalr, evalrr, evalrx]
 declare MergeCSP_def [eval, evalr, evalrr, evalrx]
 declare ParallelCSP_def [eval, evalr, evalrr, evalrx]
 declare InterleaveCSP_def [eval, evalr, evalrr, evalrx]
 
-lemma Stop_form : "`STOP`= `(\<not> ok \<and> ($tr \<le> $tr\<acute>)) \<or> ($wait \<and> ok' \<and> II\<^bsub>REL_VAR - OKAY\<^esub>) \<or> (\<not> $wait \<and> ok' \<and> \<delta>)`" by (utp_pred_auto_tac)
+lemma CSP1_rel_closure[closure]:
+  "P \<in> WF_RELATION \<Longrightarrow> CSP1(P) \<in> WF_RELATION"
+by (metis CSP1_def DesignD_extreme_point_nok(2) OrP_rel_closure R1_def R1_rel_closure TopD_rel_closure)
 
-(*
-lemma Prefix_form : "`@a`= `(\<not> ok \<and> ($tr \<le> $tr\<acute>)) \<or> ($wait \<and> ok' \<and> II\<^bsub>REL_VAR - OKAY\<^esub>) \<or> (\<not> $wait \<and> ok' \<and> $wait\<acute> \<and> (a \<notin> $ref\<acute>) \<and> ($tr \<le> $tr\<acute>)) \<or> (\<not> $wait \<and> ok' \<and> \<not> $wait\<acute> \<and> ($tr ^ \<langle>a\<rangle> = $tr\<acute>))`" 
+lemma CSP2_rel_closure[closure]: 
+  "P \<in> WF_RELATION \<Longrightarrow> CSP2(P) \<in> WF_RELATION"
+by (metis H2_def J_closure SemiR_closure)
+
+subsection {* CSP1 laws *}
+
+lemma CSP1_idempotent: "`CSP1(CSP1(P))` = `CSP1(P)`" 
+  by (utp_pred_auto_tac)
+
+lemma CSP1_monotonic: 
+  "P \<sqsubseteq> Q \<Longrightarrow> CSP1(P) \<sqsubseteq> CSP1(Q)"
+  by (utp_pred_tac)
+
+lemma CSP1_R1_commute: "CSP1 (R1 P) = R1 (CSP1 (P))"by utp_pred_auto_tac
+lemma CSP1_R2_commute: "CSP1 (R2 P) = R2 (CSP1 (P))"by(simp add:CSP1_def R2_def R2s_def usubst typing defined closure, utp_pred_auto_tac)
+lemma CSP1_R3_commute: "CSP1 (R3 P) = R3 (CSP1 (P))"by utp_pred_auto_tac
+
+lemma CSP1_AndP: 
+  "`CSP1(P \<and> Q)` = `CSP1(P) \<and> CSP1(Q)`"
+  by utp_pred_auto_tac
+
+lemma CSP1_OrP: 
+  "`CSP1(P \<or> Q)` = `CSP1(P) \<or> CSP1(Q)`"
+  by utp_pred_auto_tac
+
+lemma CSP1_CondR: 
+  "`CSP1(P \<lhd> b \<rhd> Q)` = `CSP1(P) \<lhd> b \<rhd> CSP1(Q)`"
+  by utp_pred_auto_tac
+
+lemma CSP1_Extend_OrP: 
+  "`CSP1(P) \<or> Q` = `CSP1(P \<or> Q)`"
+  by utp_pred_auto_tac
+
+lemma CSP1_R1_compose: 
+  assumes "P is R1"
+  shows "CSP1(P) = `CSP1(ok \<and> P)`"
+proof -
+  have "CSP1(P) = CSP1 (R1 P)" 
+    by (metis Healthy_simp assms)
+  thus ?thesis 
+    by(utp_pred_auto_tac)
+qed
+
+lemma ok_AndP:
+  "ok \<and> P = `ok \<and> P[true/okay]`"
+sorry
+
+lemma CSP1_R1_form: 
+  assumes "P is R1"
+  shows "CSP1(P) = `CSP1(ok \<and> P[true/okay])`"
+by (metis ok_AndP)
+
+lemma CSP1_R1_form_2: 
+  assumes "P is R1"
+  shows "CSP1(P) = `CSP1(ok \<and> P)`"
+by (metis CSP1_R1_compose assms)
+
+lemma CSP1_R1_R3_compose: 
+  assumes "P is R1"
+  shows "R3(CSP1(P)) = `(\<not>ok \<and> ($tr\<le>$tr\<acute>)) \<or> (ok \<and> $wait \<and> II) \<or> (ok \<and> \<not>$wait \<and> P[true/okay][false/wait])`"
+  apply(subst CSP1_R1_form)
+  apply(metis assms)
+  apply(simp add:R3_form_2 CSP1_def)
+  apply(utp_pred_auto_tac)
+done
+
+
+lemma CSP1_R1_R3_compose_2: 
+  assumes "P is R1"
+  shows "R3(CSP1(P)) = `(\<not>ok \<and> ($tr\<le>$tr\<acute>)) \<or> (ok \<and> $wait \<and> II) \<or> (ok \<and> \<not>$wait \<and> P)`"
+  apply(subst CSP1_R1_form_2)
+  apply(metis assms)
+  apply(simp add:R3_form CSP1_def)
+  apply(utp_pred_auto_tac)
+done
+
+lemma CSP1_R3_okay': 
+"`CSP1(ok' \<and> R3(P))` = `CSP1(R3(ok' \<and> P))`"
+by(utp_pred_auto_tac)
+
+subsection {* CSP2 laws *}
+
+lemma CSP2_idempotent: "`CSP2(CSP2(P))` = `CSP2(P)`"
+  by (metis H2_idempotent)
+
+lemma CSP2_monotonic:
+  "P \<sqsubseteq> Q \<Longrightarrow> CSP2(P) \<sqsubseteq> CSP2(Q)"
+  by (metis H2_monotone)
+
+lemma CSP1_CSP2_commute:
+  assumes "P \<in> WF_RELATION"
+  shows "CSP1 (CSP2 P) = CSP2 (CSP1 P)" 
+  apply (simp add: CSP1_def usubst typing defined closure H2_def SemiR_OrP_distr)
+  apply (metis (hide_lams, no_types) DesignD_extreme_point_nok(2) H1_H2_commute H1_def H2_def R1_H2_commute R1_def SemiR_FalseP_left TopD_rel_closure utp_pred_simps(15))
+done
+  
+lemma CSP2_form:  
+  assumes "P \<in> WF_RELATION"
+  shows "`CSP2(P)` = `P\<^sup>f \<or> ok'\<and> P\<^sup>t`"
+    apply(simp add:H2_def)
+    apply(subst J_split)
+    apply (metis assms)
+    apply(simp add:AndP_comm)
+    done
+
+lemma CSP2_R1_commute: 
+  assumes "P \<in> WF_RELATION"
+  shows "CSP2 (R1 P) = R1 (CSP2 (P))"
+by (metis R1_H2_commute assms)
+lemma CSP2_R2_commute:
+  assumes "P \<in> WF_RELATION"
+  shows"CSP2 (R2 P) = R2 (CSP2 (P))"
+by (metis H2_R2_commute assms)
+lemma CSP2_R3_commute: 
+  assumes "P \<in> WF_RELATION"
+  shows "CSP2 (R3 P) = R3 (CSP2 (P))" 
+proof -
+have "CSP2 (R3 P) = `($wait \<and> H2(II\<^bsub>rea\<^esub>)) \<or> (\<not> $wait \<and> CSP2(P))`"
+  apply(subst CSP2_form)
+  apply (metis R3_rel_closure assms)
+  apply(simp add:H2_SkipREA)
+  apply(simp add:R3_def CondR_def SkipREA_def usubst typing defined closure)
+  apply (subst CSP2_form)
+  apply (metis assms)
+  apply(utp_pred_auto_tac)
+done
+thus ?thesis by (simp add:H2_SkipREA CondR_def R3_def)
+qed
+
+lemma J_ok: 
+  "`ok \<and> J` = `ok \<and> II`"
+proof -
+  have "`ok \<and> J` = `ok \<and> ok' \<and> II\<^bsub>REL_VAR - OKAY\<^esub>`" 
+    by(simp add:J_pred_def, utp_pred_auto_tac)
+  also have "... = `(ok \<and> ($okay\<acute>=$okay)) \<and> II\<^bsub>REL_VAR - OKAY\<^esub>`" 
+    by(subst Aidb, utp_pred_auto_tac)
+  also have "... = `ok \<and> ($okay\<acute>=$okay) \<and> II\<^bsub>REL_VAR - OKAY\<^esub>`" 
+    by( utp_pred_auto_tac)
+  finally show ?thesis 
+    apply(simp add:SkipR_as_SkipRA)
+    apply(subst SkipRA_unfold[of "okay \<down>"])
+    apply(utp_pred_auto_tac)
+    apply(utp_pred_auto_tac)
+    apply(utp_pred_auto_tac)
+    apply(utp_pred_auto_tac)
+    apply(simp add:closure typing defined erasure)
+    done
+qed
+
+lemma CSP2_okay': 
+  assumes "P \<in> WF_RELATION"
+  shows "`P \<and> ok'` is CSP2"
+proof -
+  have 1:"DASHED - out REL_VAR = {}" 
+    by (metis Diff_cancel out_vars_def set_extra_simps(4))
+  have "`(P \<and> ok');J` = `P ; (ok \<and> J)`"
+    apply(subst SemiR_AndP_right_precond)
+    apply(metis assms)
+    apply (metis J_closure)
+    apply(utp_pred_auto_tac)
+    apply(simp add:urename closure typing defined)
+    done
+  also have "... = `P ; (ok \<and> II)`" 
+    by(metis J_ok)
+  also have "... = `(P \<and> ok') ; II`"
+    apply(subst SemiR_AndP_right_precond)
+    apply(metis assms)
+    apply (metis SkipR_closure)
+    apply(utp_pred_auto_tac)
+    apply(simp add:urename closure typing defined)
+    done
+  also have "... = `P \<and> ok'`"
+    apply(simp add:SkipR_as_SkipRA)
+    apply(subst SkipRA_right_unit)
+    apply(simp_all)
+    apply(subst AndP_rel_closure)
+    apply(metis assms)
+    apply(utp_pred_auto_tac)
+    apply(simp_all add:typing unrest closure defined)
+    apply(subst 1)
+    apply (metis UNREST_empty)
+    done
+  finally show ?thesis 
+    by(simp add:is_healthy_def H2_def)
+qed
+
+subsection {* CSP laws *}
+  
+lemma CSP_form: 
+assumes "P is CSP" "P \<in> WF_RELATION"
+shows "P = `(\<not>ok \<and> ($tr \<le> $tr\<acute>)) \<or> (ok \<and> $wait \<and> II) \<or> (ok \<and> \<not>$wait \<and> ($tr \<le> $tr\<acute>) \<and> R2s(P)\<^sup>f[true/okay]\<^sub>f) \<or> (ok \<and> \<not>$wait \<and> ($tr \<le> $tr\<acute>) \<and> ok' \<and> R2s(P)\<^sup>t[true/okay]\<^sub>f)`"
 proof-
-have "`@a`=  `(\<not> ok \<and> ($tr \<le> $tr\<acute>)) \<or> ($wait \<and> ok' \<and> II\<^bsub>REL_VAR - OKAY\<^esub>) \<or> (\<not> $wait \<and> ok' \<and> (((a \<notin> $ref\<acute>) \<and> ($tr \<le> $tr\<acute>)) \<lhd> $wait\<acute> \<rhd> ($tr ^ \<langle>a\<rangle> = $tr\<acute>)))`" by (simp add:prefix_def CSP1_def doA_form R3_def, utp_pred_auto_tac)
-also have "... = `(\<not> ok \<and> ($tr \<le> $tr\<acute>)) \<or> ($wait \<and> ok' \<and> II\<^bsub>REL_VAR - OKAY\<^esub>) \<or> (\<not> $wait \<and> ok' \<and> $wait\<acute> \<and> (a \<notin> $ref\<acute>) \<and> ($tr \<le> $tr\<acute>)) \<or> (\<not> $wait \<and> ok' \<and> \<not> $wait\<acute> \<and> ($tr ^ \<langle>a\<rangle> = $tr\<acute>))`"  by(simp add:CondR_def, utp_pred_auto_tac)
-finally show ?thesis ..
+  have "P = CSP P" 
+    by(metis assms(1) is_healthy_def)
+  also have "... = `R3(CSP1(R1(CSP2(R2(P)))))`"
+    by (metis CSP1_CSP2_commute CSP1_R2_commute CSP1_R3_commute CSP1_idempotent CSP_def H2_R2_commute H2_R3_commute R1_R3_commute R1_idempotent R2_R3_commute R2_def R2_rel_closure RH_def assms(2) calculation comp_apply)
+  also have "...  = `(\<not>ok \<and> ($tr \<le> $tr\<acute>)) \<or> (ok \<and> $wait \<and> II) \<or> (ok \<and> \<not>$wait \<and> ($tr \<le> $tr\<acute>) \<and> R2s(P)\<^sup>f[true/okay]\<^sub>f) \<or> (ok \<and> \<not>$wait \<and> ($tr \<le> $tr\<acute>) \<and> ok' \<and> R2s(P)\<^sup>t[true/okay]\<^sub>f)`" 
+    apply(subst CSP1_R1_R3_compose)
+    apply (metis Healthy_intro R1_idempotent)
+    apply(subst CSP2_form)
+    apply(metis assms(2) R2_rel_closure)
+    apply(simp add:R1_def usubst typing defined closure)
+    apply(utp_pred_auto_tac)
+    done
+  finally show ?thesis 
+    ..
 qed
-*)
 
-lemma Skip_form : "`SKIP`= `(\<not> ok \<and> ($tr \<le> $tr\<acute>)) \<or> ($wait \<and> ok' \<and> II\<^bsub>REL_VAR - OKAY\<^esub>) \<or> (\<not> $wait \<and> ok' \<and> (\<exists> ref .II\<^bsub>rea\<^esub>))`"by (utp_pred_auto_tac)
-lemma Chaos_form : "`CHAOS`= `(\<not> ok \<and> ($tr \<le> $tr\<acute>)) \<or> ($wait \<and> ok' \<and> II\<^bsub>REL_VAR - OKAY\<^esub> \<and> ($tr \<le> $tr\<acute>)) \<or> (\<not> $wait \<and> ($tr \<le> $tr\<acute>))`"by (utp_pred_auto_tac)
-
-lemma STOP_is_R1 : "R1 STOP = STOP "
+lemma CSP_is_RH: 
+assumes "P is CSP" "P \<in> WF_RELATION"
+shows "P is RH"
 proof -
-have "`R1( STOP )` = `CSP1( ok' \<and> R1(\<delta>))`" by utp_pred_auto_tac
-thus ?thesis by(simp add:is_healthy_def R1_\<delta> deadlock_def)
+  have "RH (P) = RH (CSP (P))" 
+    by (metis Healthy_simp assms(1))
+  also have "... = CSP P"
+    apply(simp add:CSP_def RH_def)
+    apply(subst CSP2_R1_commute)
+    apply(metis assms(2) R2_rel_closure R3_rel_closure)
+    apply(subst CSP2_R2_commute)
+    apply(metis assms(2) R3_rel_closure)
+    apply(subst CSP2_R3_commute)
+    apply(metis assms(2))
+    apply(subst CSP2_R1_commute)
+    apply(metis assms(2) R2_rel_closure R3_rel_closure)
+    apply(subst CSP2_R2_commute)
+    apply(metis assms(2) R3_rel_closure)
+    apply(subst CSP2_R3_commute)
+    apply(metis assms(2))
+    apply(simp add: CSP1_R1_commute CSP1_R2_commute CSP1_R3_commute)
+    apply(simp add:R2_R3_commute R1_R3_commute R3_idempotent R1_R2_commute R2_idempotent R1_idempotent)
+    done
+  finally show ?thesis
+    by (metis Healthy_intro Healthy_simp assms(1))
 qed
 
-lemma STOP_is_R2 : "R2 STOP = STOP" 
+lemma CSP_Design: 
+assumes "P is CSP" "P \<in> WF_RELATION"
+shows "P = `RH ( \<not>P\<^sup>f[true/okay]\<^sub>f \<turnstile> P\<^sup>t[true/okay]\<^sub>f)`"
+apply(subst CSP_form)
+apply(metis assms(1))
+apply(metis assms(2))
+apply(subst RH_form[of "`RH(\<not>P\<^sup>f[true/okay]\<^sub>f \<turnstile> P\<^sup>t[true/okay]\<^sub>f)`"])
+sorry
+
+subsection {* Stop laws *}
+
+lemma Stop_form : "`STOP`= `CSP1(R3(ok' \<and> ($tr\<acute> = $tr) \<and> $wait\<acute>))`" 
+  by(utp_pred_auto_tac)
+
+lemma Stop_expansion  :  "`STOP`= `(\<not> ok \<and> ($tr \<le> $tr\<acute>)) \<or> ($wait \<and> ok \<and> II) \<or> (\<not> $wait \<and> ok \<and> ok' \<and> ($tr\<acute> = $tr) \<and> $wait\<acute>)`" 
+  apply(simp add:Stop_form CSP1_R3_commute)
+  apply(subst CSP1_R1_R3_compose)
+  apply(utp_pred_auto_tac)
+  apply(utp_pred_auto_tac)
+done
+
+lemma Stop_is_R1 : "R1 STOP = STOP "
+apply(simp add:Stop_form CSP1_R3_commute R1_R3_commute)
+apply(utp_pred_auto_tac)
+done
+
+lemma Stop_is_R2 : "R2 STOP = STOP"
 proof - 
-have "`R2( STOP )` = `CSP1(R2( ok' \<and> \<delta>))`" by (simp add:deadlock_def CSP1_R2_commute)
-also have "... = `CSP1( ok' \<and> R2(\<delta>))`" by(simp add:R2_def R2s_def usubst typing defined closure, utp_pred_auto_tac)
-finally show ?thesis by (simp add:is_healthy_def R2_\<delta> deadlock_def)
+have "R2 STOP = `CSP1(R3(R2(ok' \<and> ($tr \<acute>=$tr) \<and> $wait \<acute>)))`"
+  by(simp add:Stop_form CSP1_R2_commute CSP1_R3_commute R2_R3_commute)
+also have "... = `CSP1(R3(ok' \<and> R1(($tr \<acute>-$tr)=\<langle>\<rangle>) \<and> $wait \<acute>))`" 
+  by(simp add:R2_def R2s_def usubst typing defined closure, utp_pred_auto_tac)
+finally show ?thesis
+  by(simp add:R1_def tr_prefix_as_nil Stop_form)
 qed
 
-lemma STOP_is_R3 : "R3 STOP = STOP" 
-proof - 
-have "`R3( STOP )` = `CSP1(R3( ok' \<and> \<delta>))`"by (simp add:deadlock_def CSP1_R3_commute)
-also have "... = `CSP1(ok' \<and> \<delta>)`" by utp_pred_auto_tac
-finally show ?thesis by (simp add:is_healthy_def deadlock_def)
-qed
+lemma Stop_is_R3 : "R3 STOP = STOP" 
+  by(simp add:Stop_form CSP1_R3_commute R3_idempotent)
+  
+lemma Stop_is_CSP1 : "CSP1 STOP = STOP" 
+  by(simp add:Stop_form CSP1_idempotent)
 
-lemma STOP_is_CSP1 : "CSP1 STOP = STOP" by(simp add:deadlock_def CSP1_idempotent)
-
-lemma STOP_is_CSP2 : "CSP2 STOP = STOP" 
+lemma Stop_is_CSP2 :
+"CSP2 STOP = STOP"
 proof -
-have "CSP2 STOP = `($okay\<acute> \<and> (II\<^bsub>rea\<^esub>[true/okay\<acute>] \<lhd> $wait \<rhd> (($tr = $tr\<acute>) \<and> $wait\<acute>))) \<or> (\<not> $okay \<and> ($tr \<le> $tr\<acute>))`"by(simp add:deadlock_def CSP2_form CSP1_def \<delta>_def R3_def usubst typing defined closure, utp_pred_auto_tac)
-also have "... = `CSP1(($okay\<acute> \<and> II\<^bsub>rea\<^esub>[true/okay\<acute>]) \<lhd> $wait \<rhd> ($okay\<acute> \<and> ($tr = $tr\<acute>) \<and> $wait\<acute>))`" by(simp add:CSP1_def, utp_pred_auto_tac)
-also have "... = `CSP1(($okay\<acute> \<and> II\<^bsub>rea\<^esub>) \<lhd> $wait \<rhd> ($okay\<acute> \<and> ($tr = $tr\<acute>) \<and> $wait\<acute>))`" 
+  have "CSP2 STOP = `CSP1(CSP2(ok' \<and> \<delta>))`"
+    apply(subst CSP1_CSP2_commute)
+    apply(subst AndP_rel_closure)
+    apply(utp_pred_auto_tac)
+    apply(simp add:\<delta>_rel_closure)
+    apply(simp_all add:StopCSP_def)
+    done
+  moreover have "`CSP2(ok' \<and> \<delta>)` = `ok' \<and> \<delta>`"
+    by (metis AndP_comm CSP2_okay' \<delta>_rel_closure is_healthy_def)
+  ultimately show ?thesis
+    by(metis StopCSP_def)
+qed
+
+lemma Stop_rel_closure[closure]: 
+  "STOP \<in> WF_RELATION"
+by(simp add:StopCSP_def closure)
+
+lemma Stop_Design_form:
+  "STOP = `RH( true \<turnstile> $wait\<acute> \<and> ($tr\<acute> = $tr))`"
+  apply(subst CSP_Design)
+  apply (metis CSP_def Healthy_intro RH_def Stop_is_CSP1 Stop_is_CSP2 Stop_is_R1 Stop_is_R2 Stop_is_R3 comp_apply)
+  apply (metis Stop_rel_closure)
+  apply (subst Stop_expansion)
+  apply (subst Stop_expansion)
+  apply(simp add:usubst typing defined closure)
+  apply( simp add:DesignD_def)
+  apply(utp_pred_auto_tac)
+done
+
+lemma Stop_precondition: 
+  "`\<not>STOP\<^sup>f\<^sub>f` = `\<not>CSP1(false)`"
+  by(simp add:Stop_expansion usubst typing defined closure CSP1_def)
+
+lemma Stop_postcondition: 
+  "`STOP\<^sup>t\<^sub>f` = `CSP1($wait\<acute> \<and> ($tr\<acute> = $tr))`"
+  apply(simp add:Stop_expansion usubst typing defined closure CSP1_def)
+  apply(utp_pred_auto_tac)
+  done
+
+lemma Stop_precondition_2: 
+  "`\<not>STOP\<^sup>f[true/okay]\<^sub>f` = `true`"
+  by(simp add:Stop_expansion usubst typing defined closure CSP1_def)
+
+lemma Stop_postcondition_2: 
+  "`STOP\<^sup>t[true/okay]\<^sub>f` = `($tr\<acute> = $tr) \<and> $wait\<acute>`"
+ by(simp add:Stop_expansion usubst typing defined closure)
+
+subsection {* Skip laws *}
+
+lemma Skip_form : "`SKIP`= `CSP1(R3(II\<^bsub>REL_VAR - {ref\<down>, ref\<down>\<acute>}\<^esub>))`" 
+proof- 
+have "`SKIP`= ` RH (CSP1( \<exists> ref. ok \<and> ($ref\<acute> = $ref) \<and> II\<^bsub>REL_VAR - {ref\<down>, ref\<down>\<acute>}\<^esub>))`"
+  apply(simp add:SkipCSP_def SkipREA_CondR_SkipR CondR_def SkipR_as_SkipRA)
+  apply(subst SkipRA_unfold[of "ref \<down>"])
+  apply(utp_pred_auto_tac)
+  apply(utp_pred_auto_tac)
+  apply(utp_pred_auto_tac) 
+  apply(utp_pred_auto_tac)
+  apply(simp add:ExistsP_OrP_dist)
+  apply(subst ExistsP_ident) back
+  apply(simp add:unrest closure typing defined)
+  apply(simp add:CSP1_def closure typing defined erasure)
+  done
+also have "... = ` RH (CSP1( \<exists> ref. ($ref\<acute> = $ref) \<and> (ok \<and> II\<^bsub>REL_VAR - {ref\<down>, ref\<down>\<acute>}\<^esub>)))`"
+  by(utp_pred_auto_tac)
+also have "... = ` RH (CSP1( (\<exists> ref. ($ref\<acute> = $ref)) \<and> (ok \<and> II\<^bsub>REL_VAR - {ref\<down>, ref\<down>\<acute>}\<^esub>)))`"
+  proof-
+  have "`\<exists> ref. ($ref\<acute> = $ref) \<and> (ok \<and> II\<^bsub>REL_VAR - {ref\<down>, ref\<down>\<acute>}\<^esub>)` = `(\<exists> ref. ($ref\<acute> = $ref)) \<and> (ok \<and> II\<^bsub>REL_VAR - {ref\<down>, ref\<down>\<acute>}\<^esub>)`"
+    apply(subst ExistsP_AndP_expand1[THEN sym])
+    apply (rule unrest) back
+    apply(simp_all add:unrest)
+    apply (rule UNREST_subset)
+    apply (rule UNREST_SkipRA)
+    apply (auto)
+  done
+  thus ?thesis 
+    by metis
+  qed
+also have "... = ` RH (CSP1(ok \<and> II\<^bsub>REL_VAR - {ref\<down>, ref\<down>\<acute>}\<^esub>))`"
+  proof-
+  have "`\<exists> ref. ($ref\<acute> = $ref)` = `true`"
+    sorry
+    thus ?thesis by (metis utp_pred_simps(6))
+  qed
+also have "... = ` RH (CSP1(II\<^bsub>REL_VAR - {ref\<down>, ref\<down>\<acute>}\<^esub>))`"
+  apply(subst CSP1_R1_compose) back
+  apply(simp_all)
+  apply(subst SkipRA_unfold[of "tr \<down>"])
+  apply(utp_pred_auto_tac)
+  apply(utp_pred_auto_tac)
+  apply(utp_pred_auto_tac)
+  apply(utp_pred_auto_tac)
+  apply(simp add:is_healthy_def R1_def)
+  apply(utp_pred_auto_tac)
+  done
+also have "... = `CSP1(RH (II\<^bsub>REL_VAR - {ref\<down>, ref\<down>\<acute>}\<^esub>))`"
+  by(simp add:RH_def CSP1_R1_commute CSP1_R2_commute CSP1_R3_commute)
+also have "... =  `CSP1 (R3 (R1 (($tr\<acute> - $tr) = \<langle>\<rangle>) \<and> II\<^bsub>REL_VAR - {ref\<down>, ref\<down>\<acute>} - {tr\<down>, tr\<down>\<acute>}\<^esub>))`"
+  apply(subst SkipRA_unfold[of "tr \<down>"])
+  apply(utp_pred_auto_tac)
+  apply(utp_pred_auto_tac)
+  apply(utp_pred_auto_tac)
+  apply(utp_pred_auto_tac)
+  apply(simp add:RH_def R2_R3_commute R1_R3_commute)
+  apply(simp add:R2_def R1_idempotent R2s_def)
+  apply(simp add:usubst typing defined closure)
+  apply(simp add:R1_def)
+  apply(utp_pred_auto_tac)
+  done
+also have "... = `CSP1 (R3 (($tr\<acute> = $tr) \<and> II\<^bsub>REL_VAR - {ref\<down>, ref\<down>\<acute>} - {tr\<down>, tr\<down>\<acute>}\<^esub>))`"
+  by(simp add:R1_def tr_prefix_as_nil)
+finally show ?thesis
+  apply(subst SkipRA_unfold[of "tr \<down>"])
+  apply(utp_pred_auto_tac)
+  apply(utp_pred_auto_tac)
+  apply(utp_pred_auto_tac)
+  apply(utp_pred_auto_tac)
+  apply(simp add:erasure closure typing defined)
+  done
+qed
+
+lemma Skip_expansion: 
+  "`SKIP`= `(\<not> ok \<and> ($tr \<le> $tr\<acute>)) \<or> (ok \<and> $wait \<and> II) \<or> (ok \<and> \<not>$wait \<and> II\<^bsub>REL_VAR - {ref\<down>, ref\<down>\<acute>}\<^esub>)`"
+apply(simp add:Skip_form CSP1_R3_commute)
+apply(subst CSP1_R1_R3_compose_2)
+apply(subst SkipRA_unfold[of "tr \<down>"])
+apply(utp_pred_auto_tac)
+apply(utp_pred_auto_tac)
+apply(utp_pred_auto_tac)
+apply(utp_pred_auto_tac)
+apply(simp add:is_healthy_def)
+apply(utp_pred_auto_tac)
+apply(utp_pred_auto_tac)
+done
+
+lemma Skip_is_R1: 
+  "SKIP is R1"
+by(utp_pred_auto_tac)
+
+lemma Skip_is_R2: 
+  "SKIP is R2"
+proof -
+have "`R2(SKIP)` = `R1 (\<not>ok) \<or> 
+  (ok \<and> $wait \<and> R1(($tr\<acute> - $tr) = \<langle>\<rangle>) \<and> II\<^bsub>REL_VAR - {tr\<down>, tr\<down>\<acute>}\<^esub>) \<or> 
+  (ok \<and> \<not> $wait \<and> R1(($tr\<acute> - $tr) = \<langle>\<rangle>) \<and> II\<^bsub>REL_VAR - {ref\<down>, ref\<down>\<acute>} - {tr\<down>, tr\<down>\<acute>}\<^esub>)`"
+apply(simp add:Skip_expansion R2_def R2s_def SkipR_as_SkipRA)
+apply(subst SkipRA_unfold[of "tr \<down>"])
+apply(utp_pred_auto_tac)
+apply(utp_pred_auto_tac)
+apply(utp_pred_auto_tac)
+apply(utp_pred_auto_tac)
+apply(subst SkipRA_unfold[of "tr \<down>"]) back
+apply(utp_pred_auto_tac)
+apply(utp_pred_auto_tac)
+apply(utp_pred_auto_tac)
+apply(utp_pred_auto_tac)
+apply(simp add:usubst typing defined closure)
+apply(utp_pred_auto_tac)
+done
+also have "... = `(\<not> ok \<and> ($tr \<le> $tr\<acute>)) \<or> 
+  (ok \<and> $wait \<and> ($tr\<acute> = $tr) \<and> II\<^bsub>REL_VAR - {tr\<down>, tr\<down>\<acute>}\<^esub>) \<or> 
+  (ok \<and> \<not> $wait \<and> ($tr\<acute> = $tr) \<and> II\<^bsub>REL_VAR - {ref\<down>, ref\<down>\<acute>} - {tr\<down>, tr\<down>\<acute>}\<^esub>)`"
+by(simp add:R1_def tr_prefix_as_nil)
+also have "... =`(\<not> ok \<and> ($tr \<le> $tr\<acute>)) \<or> 
+  (ok \<and> $wait \<and> II\<^bsub>REL_VAR\<^esub>) \<or> 
+  (ok \<and> \<not> $wait \<and> II\<^bsub>REL_VAR - {ref\<down>, ref\<down>\<acute>}\<^esub>)`"
+apply(subst SkipRA_unfold[of "tr \<down>"])back back
+apply(utp_pred_auto_tac)
+apply(utp_pred_auto_tac)
+apply(utp_pred_auto_tac)
+apply(utp_pred_auto_tac)
+apply(subst SkipRA_unfold[of "tr \<down>"])back back back
+apply(utp_pred_auto_tac)
+apply(utp_pred_auto_tac)
+apply(utp_pred_auto_tac)
+apply(utp_pred_auto_tac)
+apply(simp add:erasure closure typing defined)
+done
+finally show ?thesis 
+  by(simp add:is_healthy_def Skip_expansion SkipR_as_SkipRA)
+qed
+
+lemma Skip_is_R3: 
+  "SKIP is R3"
+by(simp add:Skip_form is_healthy_def CSP1_R3_commute R3_idempotent)
+
+lemma Skip_is_CSP1: 
+  "SKIP is CSP1"
+by(simp add:Skip_form is_healthy_def CSP1_idempotent)
+
+lemma Skip_is_CSP2: 
+  "SKIP is CSP2"
+sorry
+
+lemma Skip_rel_closure: 
+  "SKIP \<in> WF_RELATION"
+sorry
+
+lemma Skip_expansion_2:
+  "SKIP = `(\<not>ok \<and> ($tr \<le> $tr\<acute>)) \<or> (ok \<and> $wait \<and> II) \<or> (ok \<and> ok' \<and> \<not>$wait \<and> \<not>$wait\<acute> \<and> ($tr\<acute> = $tr) \<and> II\<^bsub>REL_VAR - REA\<^esub>)`"
+  apply(simp add:Skip_expansion)
+  apply(subst SkipRA_unfold[of "tr \<down>"])
+  apply(utp_pred_auto_tac)
+  apply(utp_pred_auto_tac)
+  apply(utp_pred_auto_tac)
+  apply(utp_pred_auto_tac)
+  apply(subst SkipRA_unfold[of "wait \<down>"])
+  apply(utp_pred_auto_tac)
+  apply(utp_pred_auto_tac)
+  apply(utp_pred_auto_tac)
+  apply(utp_pred_auto_tac)
+  apply(subst SkipRA_unfold[of "okay \<down>"])
+  apply(utp_pred_auto_tac)
+  apply(utp_pred_auto_tac)
+  apply(utp_pred_auto_tac)
+  apply(utp_pred_auto_tac)
   sorry
-also have "... = `CSP1($okay\<acute> \<and> (II\<^bsub>rea\<^esub> \<lhd> $wait \<rhd> (($tr = $tr\<acute>) \<and> $wait\<acute>)))`" by(utp_pred_auto_tac)
-finally show ?thesis by(simp add:deadlock_def \<delta>_def R3_def) 
+
+lemma Skip_Design_form: 
+  "SKIP = `RH( true \<turnstile> \<not>$wait\<acute> \<and> ($tr\<acute> = $tr) \<and> II\<^bsub>REL_VAR - REA\<^esub>)`"
+  apply(subst CSP_Design)
+  apply (metis (full_types) CSP_def R1_idempotent R2_def RH_def Skip_is_CSP1 Skip_is_CSP2 Skip_is_R2 Skip_is_R3 comp_def is_healthy_def)
+  apply (metis Skip_rel_closure)
+  apply (subst Skip_expansion_2)
+  apply (subst Skip_expansion_2)
+  apply(simp add:usubst typing defined closure)
+  done
+
+subsection {* Chaos laws *}
+
+lemma Chaos_form : "`CHAOS`= `CSP1(R3(R1(true)))`"
+  apply(simp add:ChaosCSP_def RH_def R2_R3_commute R1_R3_commute)
+  apply(simp add:R2_def R2s_def R1_idempotent usubst typing closure defined)
+  done
+
+lemma Chaos_expansion : "`CHAOS`= `(\<not> ok \<and> ($tr \<le> $tr\<acute>)) \<or> ($wait \<and> ok \<and> II) \<or> (\<not> $wait \<and> ($tr \<le> $tr\<acute>))`"
+apply(simp add:Chaos_form CSP1_R3_commute)
+apply(simp add:R1_def)
+apply(subst CSP1_R1_R3_compose)
+apply (metis R1_by_refinement order_refl)
+apply(utp_pred_auto_tac)
+done
+
+lemma Chaos_is_R1: 
+  "CHAOS is R1"
+by(utp_pred_auto_tac)
+
+lemma Chaos_is_R2: 
+  "CHAOS is R2"
+apply(simp add:is_healthy_def Chaos_form R1_def CSP1_R3_commute R2_R3_commute)
+apply(simp add:R2_def CSP1_def R2s_def usubst typing defined closure)
+apply(utp_pred_auto_tac)
+done
+
+lemma Chaos_is_R3: 
+  "CHAOS is R3"
+by(simp add:Chaos_form R1_def is_healthy_def CSP1_R3_commute R3_idempotent)
+
+lemma Chaos_is_CSP1: 
+  "CHAOS is CSP1"
+by(simp add:Chaos_form is_healthy_def CSP1_idempotent)
+
+lemma Chaos_is_CSP2: 
+  "CHAOS is CSP2"
+apply(simp add:Chaos_form is_healthy_def CSP1_CSP2_commute[THEN sym] closure CSP2_R3_commute CSP2_R1_commute)
+by (metis H1_left_zero H3_absorbs_H2_1 H3_def SkipD_is_H1 SkipD_rel_closure)
+
+lemma Chaos_rel_closure: 
+  "CHAOS \<in> WF_RELATION"
+by(simp add:ChaosCSP_def closure)
+
+lemma Chaos_Design_form: 
+  "CHAOS = `RH (false \<turnstile> true )`"
+apply(subst CSP_Design)
+apply (metis (full_types) CSP_def Chaos_is_CSP1 Chaos_is_CSP2 Chaos_is_R1 Chaos_is_R2 Chaos_is_R3 RH_def comp_def is_healthy_def)
+apply(metis Chaos_rel_closure)
+apply(simp add:Chaos_expansion)
+apply(simp add:usubst typing defined closure)
+apply(simp add:DesignD_def)
+apply(simp add:RH_def R2_R3_commute R1_R3_commute)
+apply(simp add:R2_def R1_idempotent R2s_def)
+apply(simp add:usubst typing defined closure)
+done
+
+subsection {*Prefix laws *}
+
+lemma Prefix_form :  
+  assumes "TR \<sharp> a" 
+  shows "`@a`= `CSP1(R3(ok' \<and> (((a \<notin> $ref\<acute>) \<and> ($tr \<le> $tr\<acute>)) \<lhd> $wait\<acute> \<rhd> ($tr ^ \<langle>a\<rangle> = $tr\<acute>))))`"
+apply(simp add:PrefixSkipCSP_def)
+apply(subst doA_form)
+apply(metis assms)
+apply (metis (hide_lams, no_types) CSP1_R3_okay' PVAR_VAR_pvdash)
+done
+
+lemma Prefix_expansion: 
+  assumes "TR \<sharp> a"
+  shows "`@a`= `(\<not> ok \<and> ($tr \<le> $tr\<acute>)) \<or> (ok \<and> $wait \<and> II) \<or> (ok \<and> ok' \<and> $wait\<acute>\<and> \<not> $wait \<and> (a \<notin> $ref\<acute>) \<and> ($tr \<le> $tr\<acute>)) \<or> (ok \<and> ok' \<and> \<not> $wait\<acute> \<and> \<not> $wait \<and> ($tr ^ \<langle>a\<rangle> = $tr\<acute>))`" 
+proof -
+have 1:"`($tr ^ \<langle>a\<rangle> = $tr\<acute>)` =`($tr ^ \<langle>a\<rangle> = $tr\<acute>) \<and> ($tr \<le> $tr\<acute>)` "
+by (metis tr_prefix_app)
+show ?thesis
+apply(subst Prefix_form)
+apply(metis assms)
+apply(simp add:CSP1_R3_commute)
+apply(subst CSP1_R1_R3_compose_2)
+apply(subst 1)
+apply(utp_pred_auto_tac)
+apply(simp add:R1_def CondR_def)
+apply(utp_pred_auto_tac)
+done
 qed
 
-lemma Seq_comp_CSP : 
-  assumes "P is CSP \<and> Q is CSP"
-  shows "P;Q = `R(\<not>(P\<^sup>f\<^sub>f;R1(true)) \<and> \<not>(P\<^sup>t\<^sub>f;Q\<^sup>f\<^sub>f) \<turnstile> P\<^sup>t\<^sub>f;Q\<^sup>t)`"
-using assms
-proof -
-from assms have "P = `R(\<not> P\<^sup>f\<^sub>f \<turnstile> P\<^sup>t\<^sub>f)`" by(metis CSP_Closure)
-moreover from assms have "Q = `R(\<not> Q\<^sup>f\<^sub>f \<turnstile> Q\<^sup>t\<^sub>f)`" by(metis CSP_Closure)
-ultimately have "P;Q = `R(\<not> P\<^sup>f\<^sub>f \<turnstile> P\<^sup>t\<^sub>f);R(\<not> Q\<^sup>f\<^sub>f \<turnstile> Q\<^sup>t\<^sub>f)`" by metis
-thus ?thesis sorry qed
+lemma Prefix_is_R1: 
+  "`@a` is R1"
+by(utp_pred_auto_tac)
 
-lemma "`a \<rightarrow> SKIP` = `@a`"
+lemma Prefix_is_R2:
+  assumes "TR \<sharp> a" 
+  shows "`@a` is R2"
 oops
 
-lemma L1 : "`CHAOS ; P` = `CHAOS`"
+lemma Prefix_is_R3: 
+  "`@a` is R3"
+proof -
+  have 1: "`do\<A>(a)` = `R3 ( do\<A>(a) )`" by(simp add:doA_is_R3)
+  have 2: "`@a` = `CSP1(R3(ok' \<and>do\<A>(a))) `"
+    apply(simp add:PrefixSkipCSP_def is_healthy_def)
+    apply(subst 1)
+    apply (metis CSP1_R3_okay' PVAR_VAR_pvdash)
+    done
+  show ?thesis 
+    apply(simp add:is_healthy_def)
+    apply(subst 2)
+    apply(subst 2)
+    apply(simp add:CSP1_R3_commute R3_idempotent)
+    done
+qed
+
+lemma Prefix_is_CSP1: 
+  "`@a` is CSP1"
+by(simp add:PrefixSkipCSP_def is_healthy_def CSP1_idempotent)
+
+lemma Prefix_is_CSP2: 
+  assumes "TR \<sharp> a" 
+  shows "`@a` is CSP2"
 sorry
 
-lemma L2 : "`STOP ; P` = `STOP`"
+lemma Prefix_rel_closure: 
+  assumes "TR \<sharp> a" 
+  shows "`@a` \<in> WF_RELATION"
 sorry
 
-lemma L3 : "(P \<sqinter> Q) \<box> S = (P \<box> S) \<sqinter> (Q \<box> s)"
+lemma Prefix_is_CSP: "`@a` is CSP" 
+sorry
+
+lemma Prefix_Design_form:
+  assumes "TR \<sharp> a" "{okay\<down>\<acute>,okay\<down>, wait\<down>} \<sharp> a"
+  shows "`@a` = `RH ( true \<turnstile> (((a \<notin> $ref\<acute>) \<and> ($tr \<le> $tr\<acute>)) \<lhd> $wait\<acute> \<rhd> ($tr ^ \<langle>a\<rangle> = $tr\<acute>)))`"
+proof -
+  have 2: "`($tr ^ \<langle>a\<rangle> = $tr\<acute>)\<^sup>t[true/okay]\<^sub>f` = `($tr ^ \<langle>a\<rangle> = $tr\<acute>)`"
+    using assms
+    apply(simp add:usubst typing defined closure UNREST_subset unrest)
+    sorry
+  have 3: "`(a \<notin> $ref\<acute>)\<^sup>t[true/okay]\<^sub>f` = `(a \<notin> $ref\<acute>)`" 
+    sorry
+  have "`@a` =  `RH (true \<turnstile> ($wait\<acute> \<and> (a \<notin> $ref\<acute>)\<^sup>t[true/okay]\<^sub>f \<and> ($tr \<le> $tr\<acute>)) \<or> (\<not> $wait\<acute> \<and> ($tr ^ \<langle>a\<rangle> = $tr\<acute>)\<^sup>t[true/okay]\<^sub>f))`"
+apply(subst CSP_Design)
+apply(metis Prefix_is_CSP)
+apply(metis Prefix_rel_closure assms)
+apply(subst Prefix_expansion)
+apply(metis assms)
+apply(subst Prefix_expansion)
+apply(metis assms)
+apply(simp add:usubst typing defined closure)
+done
+also have "... = `RH (true \<turnstile> ($wait\<acute> \<and> (a \<notin> $ref\<acute>) \<and> ($tr \<le> $tr\<acute>)) \<or> (\<not> $wait\<acute> \<and> ($tr ^ \<langle>a\<rangle> = $tr\<acute>)))`"
+  by (metis "2" "3")
+finally have 4: "`@a` =  `RH (true \<turnstile> (((a \<notin> $ref\<acute>) \<and> ($tr \<le> $tr\<acute>)) \<lhd> $wait\<acute> \<rhd> ($tr ^ \<langle>a\<rangle> = $tr\<acute>)))`"
+  by(utp_pred_auto_tac)
+show ?thesis
+  by(subst 4,simp)
+qed
+
+subsection {* Sequential composition *}
+
+lemma Seq_comp_closure: 
+assumes "P is CSP" "Q is CSP"
+shows "(P ; Q) is CSP"
+oops
+
+
+lemma Seq_comp_form: 
+assumes "P is CSP" "Q is CSP" "P \<in> WF_RELATION" "Q\<in> WF_RELATION"
+shows "(P ; Q) = `RH (\<not>(P\<^sup>f\<^sub>f;R1(true)) \<and> \<not>(P\<^sup>t\<^sub>f[false/wait\<acute>];(Q\<^sup>f\<^sub>f)) \<turnstile> P\<^sup>t\<^sub>f;(R3(Q\<^sup>t\<^sub>f)))`"
+sorry
+
+lemma Seq_comp_form_2: 
+assumes "P is CSP" "Q is CSP" "P \<in> WF_RELATION" "Q\<in> WF_RELATION"
+shows "(P ; Q) = `RH (\<not>(P\<^sup>f[true/okay]\<^sub>f;R1(true)) \<and> \<not>(P\<^sup>t[true/okay]\<^sub>f[false/wait\<acute>];(Q\<^sup>f[true/okay]\<^sub>f)) \<turnstile> P\<^sup>t[true/okay]\<^sub>f;(II\<^bsub>REL_VAR-OKAY\<^esub> \<lhd> $wait \<rhd> (Q\<^sup>t[true/okay]\<^sub>f)))`"
+sorry
+
+subsection {* Prefixed laws *}
+
+lemma 
+  assumes "TR \<sharp> a" "{okay\<down>\<acute>, okay\<down>, wait\<down>} \<sharp> a"
+  shows "`a \<rightarrow> SKIP` = `@a`" 
+apply(simp add:PrefixCSP_def)
+apply(subst Prefix_Design_form) back
+apply(metis assms(1))
+apply(metis assms(2))
+apply(subst Seq_comp_form)
+apply(metis Prefix_is_CSP)
+apply (metis (full_types) CSP_def Healthy_intro Healthy_simp R1_idempotent R2_R3_commute R2_def RH_def Skip_is_CSP1 Skip_is_CSP2 Skip_is_R2 Skip_is_R3 o_eq_dest_lhs)
+apply(subst Prefix_rel_closure)
+apply(simp_all add:assms Skip_rel_closure)
+apply(subst Prefix_expansion)
+apply(metis assms(1))
+apply(subst Prefix_expansion)
+apply(metis assms(1))
+apply(subst Prefix_expansion)
+apply(metis assms(1))
+apply(simp add:Skip_expansion_2)
+oops
+
+subsection {*CSP laws*}
+
+lemma L1 : 
+  assumes "P is CSP" "P \<in> WF_RELATION"
+  shows "`CHAOS ; P` = `CHAOS`"
+proof -
+  have a: "`((\<not> ok \<and> ($tr \<le> $tr\<acute>)) \<or> ($tr \<le> $tr\<acute>)) ; R1 (true)` = `($tr \<le> $tr\<acute>)`"
+  proof -
+    have 1: "`(\<not> ok \<and> ($tr \<le> $tr\<acute>)) \<or> ($tr \<le> $tr\<acute>)` = `($tr \<le> $tr\<acute>)`" 
+      by(utp_pred_auto_tac)
+    have "`((\<not> ok \<and> ($tr \<le> $tr\<acute>)) \<or> ($tr \<le> $tr\<acute>)) ; R1 (true)` =`($tr \<le> $tr\<acute>);($tr \<le> $tr\<acute>)`"
+      by(simp add: R1_def "1")
+    thus ?thesis 
+      by(simp add: tr_leq_trans)
+  qed
+show ?thesis
+apply(subst Chaos_Design_form) back
+apply(subst Seq_comp_form)
+apply (metis CSP_def Chaos_is_CSP1 Chaos_is_CSP2 Chaos_is_R1 Chaos_is_R2 Chaos_is_R3 Healthy_comp R_intro is_healthy_def)
+apply(metis assms(1))
+apply (metis Chaos_rel_closure)
+apply (metis assms(2))
+apply(simp add:Chaos_expansion)
+apply(simp add:usubst typing defined closure)
+apply(simp add:DesignD_def)
+apply(subst "a")
+apply(simp add:RH_def R1_R2_commute R1_R3_commute)
+apply(simp add:R1_def)
+apply(utp_pred_auto_tac)
+done
+qed
+
+thm DesignD_composition
+
+lemma L2 : 
+assumes "P is CSP" "P \<in> WF_RELATION"
+shows "`STOP ; P` = `STOP`"
+
+
+
+proof -
+  have 1: "`STOP\<^sup>f[true/okay]\<^sub>f` = `false`" by (metis Stop_precondition_2 utp_pred_simps(2) utp_pred_simps(3))
+  have 2: "`STOP\<^sup>t[true/okay]\<^sub>f` = `($tr = $tr\<acute>) \<and> $wait\<acute>`" by (metis EqualP_sym Stop_postcondition_2)
+  have " `STOP ; P` = `RH (true \<turnstile> (($tr = $tr\<acute>) \<and> $wait\<acute>) ; (II\<^bsub>REL_VAR-OKAY\<^esub> \<lhd> $wait \<rhd> (P\<^sup>t[true/okay]\<^sub>f)))`"
+    apply(subst Seq_comp_form_2)
+    apply (metis CSP_def Healthy_intro RH_def Stop_is_CSP1 Stop_is_CSP2 Stop_is_R1 Stop_is_R2 Stop_is_R3 comp_apply)
+    apply(metis assms(1))
+    apply(metis Stop_rel_closure)
+    apply(metis assms(2))
+    apply(subst 1)
+    apply(subst 2)
+    apply(subst 2)
+    apply(subst SemiR_FalseP_left)
+    apply(simp add:usubst typing defined closure)
+    done
+  also have "... = `RH (true \<turnstile> ($tr = $tr\<acute>) ; ($wait \<and> (II\<^bsub>REL_VAR-OKAY\<^esub> \<lhd> $wait \<rhd> (P\<^sup>t[true/okay]\<^sub>f))))`"
+    apply(subst SemiR_AndP_right_precond)
+    apply(simp add:closure unrest typing defined)
+    defer
+    apply(utp_pred_auto_tac)
+    apply (simp add:urename typing defined closure)
+    apply(subst CondR_rel_closure)
+    apply(simp_all add:closure)
+    sorry
+  also have "... = `RH (true \<turnstile> ($tr = $tr\<acute>) ; ($wait \<and> II\<^bsub>REL_VAR-OKAY\<^esub>))`"
+    proof -
+      have "`($wait \<and> (II\<^bsub>REL_VAR-OKAY\<^esub> \<lhd> $wait \<rhd> (P\<^sup>t[true/okay]\<^sub>f)))` = `$wait \<and> II\<^bsub>REL_VAR-OKAY\<^esub>`"by utp_pred_auto_tac
+      thus ?thesis by metis
+    qed
+  also have "... = `RH (true \<turnstile> (($tr = $tr\<acute>) \<and> $wait\<acute>) ; II)`"
+    apply(subst SemiR_AndP_right_precond)
+    sorry
+  also have "... =`RH (true \<turnstile> ($tr = $tr\<acute>) \<and> $wait\<acute>)`"
+    by (metis SemiR_SkipR_right)
+  also have "... = STOP" 
+    by (metis AndP_comm EqualP_sym Stop_Design_form)
+  finally show ?thesis
+    ..
+qed
+
+lemma L3 : "(P \<sqinter> Q) \<box> S = (P \<box> S) \<sqinter> (Q \<box> S)"
 oops
 
 lemma L4 : "P \<sqinter> (Q \<box> S) = (P \<sqinter> Q) \<box> (P \<sqinter> S)"
