theories/theories/utp_reactive.thy
@@ -75,13 +75,99 @@ lemma R2s_rel_closure [closure]:
   "P \<in> WF_RELATION \<Longrightarrow> R2s(P) \<in> WF_RELATION"
   by (simp add:R2s_def unrest typing defined closure)
 
-lemma R2_closure [closure]:
+lemma R2_rel_closure [closure]:
   "P \<in> WF_RELATION \<Longrightarrow> R2(P) \<in> WF_RELATION"
   by (simp add:R2_def closure)
 
-lemma R3_closure [closure]:
+lemma R3_rel_closure [closure]:
   "P \<in> WF_RELATION \<Longrightarrow> R3(P) \<in> WF_RELATION"
   by (simp add:R3_def closure)
+
+lemma RH_rel_closure [closure]: 
+  "P \<in> WF_RELATION \<Longrightarrow> RH(P) \<in> WF_RELATION"
+  by (simp add:RH_def closure)
+
+subsection {* Sorried Laws *}
+
+(* Trace sequence relation *)
+lemma Aida : "`(($tr \<le> $tr\<acute>) ; (\<not>ok \<and> $wait \<and> ($tr \<le> $tr\<acute>)))`=`($tr \<le> $tr\<acute>)`"
+proof- 
+  have "`(($tr \<le> $tr\<acute>) ; (\<not>ok \<and> $wait \<and> ($tr \<le> $tr\<acute>)))`= `($tr \<le> $tr\<acute>) ; ($wait \<and> ($tr \<le> $tr\<acute>))`"
+    apply(subst SemiR_extract_variable[where x="okay \<down>"])
+    apply (metis R1_def R1_rel_closure TrueP_rel_closure utp_pred_simps(6))
+    apply (metis AndP_rel_closure DesignD_extreme_point_nok(2) MkPlainP_UNDASHED PUNDASHED_WF_CONDITION R1_def R1_rel_closure TopD_rel_closure WF_CONDITION_WF_RELATION)
+    apply (metis MkPlain_UNDASHED PVAR_VAR_MkPVAR)
+    apply(simp add:usubst typing closure defined unrest)
+    apply(subst BoolType_aux_var_split_exists)
+    apply(simp_all add:typing)
+    apply(simp add: usubst typing closure defined erasure unrest)
+    done
+  also have "... = `($tr \<le> $tr\<acute>) ; (($tr \<le> $tr\<acute>) \<and> $wait)`"
+    by (metis AndP_comm)
+  also have "... = `\<exists> wait\<acute>\<acute>\<acute> . ($tr \<le> $tr\<acute>) ; (($tr \<le> $tr\<acute>) \<and> $wait\<acute>\<acute>\<acute>)`"
+    apply(subst SemiR_extract_variable[where x="wait \<down>"])
+    apply (metis R1_def R1_rel_closure TrueP_rel_closure utp_pred_simps(6))
+    apply (smt AndP_comm MkPlainP_UNDASHED PUNDASHED_WF_CONDITION R1_def R1_rel_closure WF_CONDITION_WF_RELATION)
+    apply (metis MkPlain_UNDASHED PVAR_VAR_MkPVAR)
+    apply(simp add:usubst typing closure defined unrest)
+    done
+  also have "... = `\<exists> wait\<acute>\<acute>\<acute> . ( ($tr \<le> $tr\<acute>) ; ($tr \<le> $tr\<acute>) )\<and> $wait\<acute>\<acute>\<acute>`"
+    sorry
+  also have "... = `( ($tr \<le> $tr\<acute>) ; ($tr \<le> $tr\<acute>) )\<and> (\<exists> wait\<acute>\<acute>\<acute> . $wait\<acute>\<acute>\<acute>)`" 
+    sorry
+  also have "... = `($tr \<le> $tr\<acute>) ; ($tr \<le> $tr\<acute>)`"
+    sorry
+  finally show ?thesis 
+    by (metis tr_leq_trans)
+qed
+    
+lemma Aidb : "`$okay \<and> ($okay\<acute> = $okay)` = `$okay \<and> $okay\<acute>`" by (utp_pred_auto_tac)
+lemma Aidc : "`$wait \<and> ($wait\<acute> = $wait)` = `$wait \<and> $wait\<acute>`" by (utp_pred_auto_tac)
+lemma Aidd : "`II\<^bsub>REL_VAR - OKAY\<^esub>\<^sub>t`=`$wait\<acute> \<and> II\<^bsub>REL_VAR - OKAY - {wait\<down>, wait\<down>\<acute>}\<^esub>`"
+  apply (subst SkipRA_unfold[of "wait \<down>"])
+  apply (simp_all)
+  apply (metis MkPlain_UNDASHED PVAR_VAR_MkPVAR)
+  apply (metis MkPlain_UNDASHED PVAR_VAR_MkPVAR UNDASHED_dash_DASHED)
+  apply (metis MkPlainP_UNDASHED PVAR_VAR_PUNDASHED_UNDASHED) 
+  apply (utp_pred_auto_tac)
+  apply (simp add: usubst typing closure defined)
+  apply (subst VarP_EqualP_aux)
+  apply (simp_all add:typing erasure)
+done
+
+subsection {* SkipREA Laws *}
+
+(* Additional lemmas *)
+
+lemma SkipRA_is_R1 : 
+  "`R1(II\<^bsub>REL_VAR - OKAY\<^esub>)` = `II\<^bsub>REL_VAR - OKAY\<^esub>`"
+  by (auto simp add:var_dist closure eval)
+
+lemma tr_conserved_is_R1 : "`R1($tr\<acute> = $tr)` = `($tr\<acute> = $tr)`" 
+  by (simp add:R1_def, utp_pred_auto_tac)
+
+lemma R1_monotonic: "P \<sqsubseteq> Q \<Longrightarrow> R1(P) \<sqsubseteq> R1(Q)" 
+  by utp_pred_tac
+
+(*L1 H1-wait-okay' *)
+
+lemma H1_wait_true: 
+  "(H1(P))\<^sub>t = H1(P\<^sub>t)"
+by(utp_pred_auto_tac)
+
+lemma H1_wait_false: 
+  "(H1(P))\<^sub>f = H1(P\<^sub>f)"
+by(utp_pred_auto_tac)
+
+lemma H1_okay'_true: 
+  "(H1(P))\<^sup>t = H1(P\<^sup>t)"
+by(utp_pred_auto_tac)
+
+lemma H1_okay'_false: 
+  "(H1(P))\<^sup>f = H1(P\<^sup>f)"
+by(utp_pred_auto_tac)
+
+(*L3 II_rea-II_rel-conditional *)
 
 lemma SkipREA_CondR_SkipR: 
   "`II\<^bsub>rea\<^esub>` = `II \<lhd> ok \<rhd> ($tr \<le> $tr\<acute>)`"
@@ -112,21 +198,80 @@ proof -
   finally show ?thesis ..
 qed
 
-lemma H1_SkipREA: 
-  "`H1(II\<^bsub>rea\<^esub>)` = `H1(II)`"
+(*L2 II_rea-II_rel *)
+
+lemma SkipREA_SkipR: 
+  "`II\<^bsub>rea\<^esub>` = `(\<not> ok \<and> ($tr \<le> $tr\<acute>)) \<or> II`"
 proof -
-  have "`H1(II\<^bsub>rea\<^esub>)` = `ok \<Rightarrow> II\<^bsub>rea\<^esub>`"
-    by (simp add:H1_def)
-
-  also have "... = `ok \<Rightarrow> (II \<lhd> ok \<rhd> ($tr \<le> $tr\<acute>))`"
-    by (simp add:SkipREA_CondR_SkipR)
-
-  also have "... = `ok \<Rightarrow> II`"
-    by (metis (lifting, no_types) CondR_true_cond ImpliesP_export)
-
-  finally show ?thesis
-    by (simp add:H1_def)
+  have "`II\<^bsub>rea\<^esub>` = `(\<not> ok \<and> ($tr \<le> $tr\<acute>)) \<or> (ok \<and> II)`" by(simp add: OrP_comm SkipREA_CondR_SkipR CondR_def)
+  also have "... = `(\<not> ok \<and> ($tr \<le> $tr\<acute>)) \<or> (\<not> ok \<and> ($tr \<le> $tr\<acute>) \<and> II) \<or> (ok \<and> II)`" by utp_pred_auto_tac
+  also have "... = `(\<not> ok \<and> ($tr \<le> $tr\<acute>)) \<or> (\<not> ok \<and> II) \<or> (ok \<and> II)`"
+  proof -
+    have "`($tr \<le> $tr\<acute>) \<and> II` = `R1(II)`"
+      by utp_pred_auto_tac
+    also have "... = `R1($tr\<acute> = $tr) \<and> II\<^bsub>REL_VAR - {tr\<down>,tr\<down>\<acute>}\<^esub>`"
+      apply(simp add:SkipR_as_SkipRA)
+      apply(subst SkipRA_unfold[of "tr \<down>"])
+      apply(simp_all)
+      apply(metis MkPlain_UNDASHED PVAR_VAR_MkPVAR)
+      apply(metis MkPlain_UNDASHED PVAR_VAR_MkPVAR UNDASHED_dash_DASHED)
+      apply(metis MkPlain_UNDASHED PVAR_VAR_MkPVAR)
+      apply(simp add:typing closure defined erasure)
+      apply(utp_pred_auto_tac)
+      done
+    also have "... = `($tr\<acute> = $tr) \<and> II\<^bsub>REL_VAR - {tr\<down>,tr\<down>\<acute>}\<^esub>`"
+      by(utp_pred_auto_tac)
+    finally have "`($tr \<le> $tr\<acute>) \<and> II` = `II`" 
+      apply(simp add: SkipR_as_SkipRA)
+      apply(subst SkipRA_unfold[of "tr \<down>"]) back
+      apply(simp_all)
+      apply(metis MkPlain_UNDASHED PVAR_VAR_MkPVAR)
+      apply(metis MkPlain_UNDASHED PVAR_VAR_MkPVAR UNDASHED_dash_DASHED)
+      apply(metis MkPlain_UNDASHED PVAR_VAR_MkPVAR)
+      apply(simp add:typing closure defined erasure)
+      done 
+    thus ?thesis by metis
+  qed
+  finally show ?thesis by utp_pred_auto_tac
 qed
+
+(*L4 okay-II_rea-II_rel *)
+
+lemma ok_SkipREA_SkipR : 
+  "`ok \<and> II\<^bsub>rea\<^esub>` = `ok \<and> II`"
+proof -
+  have "`ok \<and> II\<^bsub>rea\<^esub>` = `ok \<and> ok' \<and> II\<^bsub>REL_VAR - OKAY\<^esub>`" 
+    by(utp_pred_auto_tac)
+  also have "... = `ok \<and> II\<^bsub>REL_VAR\<^esub>`" 
+  proof -
+      have "`ok \<and> ok'` = `ok \<and> ($okay\<acute> = $okay)`"
+        by (metis Aidb)
+      thus ?thesis
+        apply(simp add: SkipRA_unfold[of "okay \<down>"] closure erasure typing defined)
+        apply(utp_pred_auto_tac)
+        done
+  qed
+  finally show ?thesis 
+    by (metis SkipR_as_SkipRA)
+qed
+
+(*L5 okay-II_rea-sequence-unit *)
+
+lemma okay_SkipREA_sequence_unit : 
+assumes 
+  "P \<in> WF_RELATION"
+shows
+  "`(ok \<and> II\<^bsub>rea\<^esub>) ; P` = `ok \<and> P`"
+proof -
+  have "`(ok \<and> II\<^bsub>rea\<^esub>) ; P` = `(ok \<and> II) ; P`" 
+    by (metis ok_SkipREA_SkipR)
+  also  have "... = `ok \<and> (II ; P)`"
+    by (subst SemiR_AndP_left_precond, simp_all add:SkipR_closure assms MkPlainP_UNDASHED PUNDASHED_WF_CONDITION)
+  finally show ?thesis 
+    by(simp)
+qed
+
+(*L6 II_rea-H2 *)
 
 lemma H2_SkipREA:
   "`H2(II\<^bsub>rea\<^esub>)` = `II\<^bsub>rea\<^esub>`"
@@ -147,31 +292,128 @@ proof -
   finally show ?thesis .
 qed
 
+(*L7 H1-II_rea-II_rel *)
+
+lemma H1_SkipREA: 
+  "`H1(II\<^bsub>rea\<^esub>)` = `H1(II)`"
+proof -
+  have "`H1(II\<^bsub>rea\<^esub>)` = `ok \<Rightarrow> II\<^bsub>rea\<^esub>`"
+    by (simp add:H1_def)
+
+  also have "... = `ok \<Rightarrow> (II \<lhd> ok \<rhd> ($tr \<le> $tr\<acute>))`"
+    by (simp add:SkipREA_CondR_SkipR)
+
+  also have "... = `ok \<Rightarrow> II`"
+    by (metis (lifting, no_types) CondR_true_cond ImpliesP_export)
+
+  finally show ?thesis
+    by (simp add:H1_def)
+qed
+
+subsection {* R1 Laws *}
+
+(* L1 R1-idempotent *)
+
 lemma R1_idempotent:
   "R1(R1(P)) = R1(P)"
   by (utp_rel_tac)
+
+(* L2 R1-\<and> *)
 
 lemma R1_AndP:
   "`R1(P \<and> Q)` = `R1(P) \<and> R1(Q)`"
   by (utp_pred_auto_tac)
 
+(* L3 R1-\<or> *)
+
 lemma R1_OrP:
   "`R1(P \<or> Q)` = `R1(P) \<or> R1(Q)`"
   by (utp_pred_auto_tac)
   
+(* L4 R1-extend-\<and> *)
+
+lemma R1_extend_AndP : 
+  "`R1(P) \<and> Q` = `R1(P \<and> Q)`"
+  by (utp_pred_auto_tac)
+
+(* L5 R1-conditional *)
+
 lemma R1_CondR:
   "`R1(P \<lhd> b \<rhd> Q)` = `R1(P) \<lhd> b \<rhd> R1(Q)`"
-by (utp_pred_auto_tac)
+  by (utp_pred_auto_tac)
+
+(* L6 R1-negate-R1 *)
+
+lemma R1_negate_R1: 
+  "`R1(\<not>R1(P))` = `R1(\<not>P)`"
+  by(utp_pred_auto_tac)
   
+(* L7 R1-wait-okay' *)
+
+lemma R1_wait_true: 
+  "(R1(P))\<^sub>t = R1(P\<^sub>t)"
+by(utp_pred_auto_tac)
+
+lemma R1_wait_false: 
+  "(R1(P))\<^sub>f = R1(P\<^sub>f)"
+by(utp_pred_auto_tac)
+
+lemma R1_okay'_true: 
+  "(R1(P))\<^sup>t = R1(P\<^sup>t)"
+by(utp_pred_auto_tac)
+
+lemma R1_okay'_false: 
+  "(R1(P))\<^sup>f = R1(P\<^sup>f)"
+by(utp_pred_auto_tac)
+
+(* L8 II_rel-R1 *)
+
 lemma R1_SkipR:
   "R1(II) = II"
   by (auto simp add:eval closure)
+
+(* L9 II_rea-R1 *)
+
+lemma R1_SkipREA:
+  "`R1(II\<^bsub>rea\<^esub>)` = `II\<^bsub>rea\<^esub>`"
+  by (auto simp add:eval closure)
+
+lemma R1_tr_leq_tr':
+  "`R1($tr \<le> $tr\<acute>)` = `$tr \<le> $tr\<acute>`"
+  by (simp add:R1_def)
+
+lemma SkipREA_is_R1:
+  "`R1(II\<^bsub>rea\<^esub>)` = `II\<^bsub>rea\<^esub>`"
+  by (simp add:SkipREA_CondR_SkipR R1_CondR R1_SkipR R1_tr_leq_tr')
+
+(* L10 R1-\<and>-closure *)
+
+lemma R1_AndP_closure: 
+assumes "P is R1" "Q is R1"
+shows "`(P \<and> Q)` is R1"
+by (metis Healthy_intro Healthy_simp R1_extend_AndP assms(1))
+
+(* L11 R1-\<or>-closure *)
+
+lemma R1_OrP_closure: 
+assumes "P is R1" "Q is R1"
+shows "`(P \<or> Q)` is R1"
+by (metis R1_OrP assms(1) assms(2) is_healthy_def)
+
+(* L12 R1-conditional-closure *)
+
+lemma R1_CondR_closure: 
+assumes "P is R1" "Q is R1"
+shows "`(P \<lhd> b \<rhd> Q)` is R1"
+by (metis Healthy_intro Healthy_simp R1_CondR assms(1) assms(2))
+
+(* L13 R10-sequence-closure *)
 
 lemma R1_by_refinement:
   "P is R1 \<longleftrightarrow> `$tr \<le> $tr\<acute>` \<sqsubseteq> P" 
   by (utp_pred_auto_tac)
 
-theorem R1_SemiR [closure]:
+theorem R1_SemiR_closure [closure]:
   assumes
     "P \<in> WF_RELATION" "Q \<in> WF_RELATION"
     "P is R1" "Q is R1"
@@ -184,20 +426,339 @@ theorem R1_SemiR [closure]:
   apply (simp add:tr_leq_trans)
 done
 
-lemma R1_tr_leq_tr':
-  "`R1($tr \<le> $tr\<acute>)` = `$tr \<le> $tr\<acute>`"
-  by (simp add:R1_def)
+(* L14 II_rea-R1-H1 *)
+
+lemma SkipREA_R1_H1: 
+  "`II\<^bsub>rea\<^esub>` = `R1(H1(II\<^bsub>rea\<^esub>))`"
+proof -
+  from SkipREA_is_R1 have "`II\<^bsub>rea\<^esub>` = `R1(II\<^bsub>rea\<^esub>)`" 
+    ..
+  thus ?thesis 
+    by(utp_pred_auto_tac)
+qed
+
+(* L15 R1-H2-commutativity *)
 
 lemma R1_H2_commute:
-  "P \<in> WF_RELATION \<Longrightarrow> H2(R1(P)) = R1(H2(P))"
+  assumes "P \<in> WF_RELATION"
+  shows "H2(R1(P)) = R1(H2(P))"
   apply (simp add: H2_def J_split unrest closure)
+  apply (subst J_split)
+  apply (metis R1_rel_closure assms)
+  apply (subst J_split)
+  apply (metis assms)
   apply (simp add: R1_def usubst typing defined)
   apply (utp_pred_auto_tac)
 done
 
-lemma SkipRA_is_R1 : 
-  "`R1(II\<^bsub>REL_VAR - OKAY\<^esub>)` = `II\<^bsub>REL_VAR - OKAY\<^esub>`"
-  by (auto simp add:var_dist closure eval)
+subsection {* R2 Laws *}
+
+(* L3 R2-idempotent *)
+
+lemma R2s_idempotent: "`R2s(R2s(P))` = `R2s(P)`"
+  apply (simp add:R2s_def)
+  apply (subst SubstP_twice_3) back
+  apply (simp_all add:typing defined closure unrest)
+  apply (simp add:usubst typing defined closure)
+done
+
+lemma R2s_destroys_R1: "R2s (R1 P) = R2s P" 
+  by (simp add:R2s_def R1_def usubst closure typing defined)
+
+lemma R2_idempotent: "`R2(R2(P))` = `R2(P)`" 
+  by (simp add:R2_def R2s_destroys_R1 R2s_idempotent)
+
+(* L4 R2-\<and>-closure *)
+
+lemma R2s_AndP: 
+  "`R2s(P \<and> Q)` = `R2s(P) \<and> R2s(Q)`" 
+  by (utp_pred_auto_tac)
+
+lemma R2_AndP: "`R2(P \<and> Q)` = `R2(P) \<and> R2(Q)`"
+  by (utp_pred_auto_tac)
+
+lemma R2_AndP_closure: 
+assumes "P is R2" "Q is R2"
+shows "`P \<and> Q` is R2"
+by (metis R2_AndP assms(1) assms(2) is_healthy_def)
+
+(* L5 R2-\<or>-closure *)
+
+lemma R2s_OrP: 
+  "`R2s(A \<or> C)` = `R2s(A) \<or> R2s(C)`" 
+  by (utp_pred_auto_tac)
+
+lemma R2_OrP: "`R2(P \<or> Q)` = `R2(P) \<or> R2(Q)`"
+  by (utp_pred_auto_tac)
+
+lemma R2_OrP_closure: 
+assumes "P is R2" "Q is R2"
+shows "`P \<or> Q` is R2"
+by (metis R2_OrP assms(1) assms(2) is_healthy_def)
+
+(* L7 R2-cond-closure-2 *)
+
+lemma R2s_CondR: 
+  "`R2s(P \<lhd> b \<rhd> Q)` = `R2s(P) \<lhd> R2s(b) \<rhd> R2s(Q)`"
+  by (utp_pred_auto_tac)
+
+lemma R2_CondR: 
+  "`R2(P \<lhd> b \<rhd> Q)` =`R2(P) \<lhd> R2s(b) \<rhd> R2(Q)`" 
+  by (utp_pred_auto_tac)
+
+lemma R2_CondR_alt: 
+  "`R2(P \<lhd> b \<rhd> Q)` =`R2(P) \<lhd> R2(b) \<rhd> R2(Q)`" 
+  by (utp_pred_auto_tac)
+
+lemma R2_negate: 
+  "`R2(\<not> b)` = `R1(\<not>R2(b))`"
+by(utp_pred_auto_tac)
+
+lemma R2_CondR_closure_2: 
+assumes "P is R2" "Q is R2" "b is R2"
+shows "`P \<lhd> b \<rhd> Q` is R2"
+using assms
+proof -
+  have "`R2(P \<lhd> b \<rhd> Q)`  = `(R2(b) \<and> R2(P)) \<or> (R1(\<not> R2(b)) \<and> R2(Q))`"
+    by(simp add:CondR_def R2_OrP R2_AndP R2_negate)
+  also have "... = `(R2(b) \<and> R2(P)) \<or> (\<not> R2(b) \<and> R2(Q))`"
+    by(utp_pred_auto_tac)
+  also from assms have "... = `(b \<and> P) \<or> (\<not> b \<and> Q)`" 
+    by(simp add:is_healthy_def)
+  finally show ?thesis
+    by (simp add:is_healthy_def CondR_def)
+qed
+
+(* L6 R2-cond-closure-1 *)
+
+lemma tr_conserved_is_R2 : "`R2($tr\<acute> = $tr)` = `($tr\<acute> = $tr)`"
+  apply(simp add:R2_def R2s_def R1_def usubst typing defined closure)
+  apply (metis EqualP_sym tr_prefix_as_nil)
+done
+
+lemma R2_CondR_closure_1: 
+assumes "P is R2" "Q is R2"
+shows "`P \<lhd> ($tr\<acute> = $tr) \<rhd> Q` is R2"
+by(subst R2_CondR_closure_2, simp_all add:assms, simp add:is_healthy_def tr_conserved_is_R2)
+
+(* L9 R2-composition *)
+(*R2 *)
+lemma R2_sequential_composition: 
+  assumes "P \<in> WF_RELATION" "Q \<in> WF_RELATION"
+  shows "`R2(P);R2(Q)` = `R2(P ; R2(Q))`"
+proof -
+have "`R2(P;R2(Q))` = `R2(\<exists> tr\<acute>\<acute>\<acute> . (P[$tr\<acute>\<acute>\<acute>/tr\<acute>]);(R2(Q)[$tr\<acute>\<acute>\<acute>/tr]))`"
+  apply(subst SemiR_extract_variable[where x="tr \<down>"])
+  apply (metis assms(1))
+  apply (metis R2_rel_closure assms(2))
+  apply (metis MkPlain_UNDASHED PVAR_VAR_MkPVAR)
+  apply (simp add:closure typing defined erasure)
+  done
+also have "... = `R1(
+
+(\<exists> tr\<acute>\<acute>\<acute> . P[$tr\<acute>\<acute>\<acute>/tr\<acute>];(Q[\<langle>\<rangle>/tr][($tr\<acute> - $tr)/tr\<acute>] \<and>  ($tr \<le> $tr\<acute>))[$tr\<acute>\<acute>\<acute>/tr])
+
+[\<langle>\<rangle>/tr][($tr\<acute> - $tr)/tr\<acute>]
+
+)`"
+  by(simp add:R2_def R1_def R2s_def)
+also have "... = `R1(\<exists> tr\<acute>\<acute>\<acute> . (P[$tr\<acute>\<acute>\<acute>/tr\<acute>];(Q[\<langle>\<rangle>/tr][($tr\<acute> - $tr)/tr\<acute>] \<and>  ($tr \<le> $tr\<acute>))[$tr\<acute>\<acute>\<acute>/tr])[\<langle>\<rangle>/tr][($tr\<acute> - $tr)/tr\<acute>])`"
+  apply(subst SubstP_ExistsP)
+  apply(simp_all add:unrest typing defined closure)
+  apply(subst SubstP_ExistsP)
+  apply(simp_all add:unrest typing defined closure)
+  done
+also have "... = `R1(\<exists> tr\<acute>\<acute>\<acute> . (P[\<langle>\<rangle>/tr][$tr\<acute>\<acute>\<acute>/tr\<acute>];(Q[\<langle>\<rangle>/tr][(($tr\<acute> - $tr) - $tr\<acute>\<acute>\<acute>)/tr\<acute>] \<and>  ($tr\<acute>\<acute>\<acute> \<le> ($tr\<acute> - $tr)))))`"
+   apply(subst SubstP_SemiR_left[of "tr \<down>"])
+   apply (metis MkPlain_UNDASHED PVAR_VAR_MkPVAR)
+   apply(simp_all add:unrest typing defined closure)
+   sorry (*distributing substitution through SemiR *)
+also have "... = `R1(\<exists> tr\<acute>\<acute>\<acute>\<acute> . \<exists> tr\<acute>\<acute>\<acute> . $tr\<acute>\<acute>\<acute>\<acute> = $tr^$tr\<acute>\<acute>\<acute> \<and> (P[\<langle>\<rangle>/tr][($tr\<acute>\<acute>\<acute>\<acute> - $tr)/tr\<acute>];(Q[\<langle>\<rangle>/tr][(($tr\<acute> - $tr) - ($tr\<acute>\<acute>\<acute>\<acute> - $tr))/tr\<acute>] \<and>  (($tr\<acute>\<acute>\<acute>\<acute> - $tr) \<le> ($tr\<acute> - $tr)))))`" sorry (*introduce fresh quantifier *)
+also have "... = `R1(\<exists> tr\<acute>\<acute>\<acute>\<acute> . (P[\<langle>\<rangle>/tr][($tr\<acute>\<acute>\<acute>\<acute> - $tr)/tr\<acute>];(Q[\<langle>\<rangle>/tr][(($tr\<acute> - $tr) - ($tr\<acute>\<acute>\<acute>\<acute> - $tr))/tr\<acute>] \<and>  (($tr\<acute>\<acute>\<acute>\<acute> - $tr) \<le> ($tr\<acute> - $tr)))))`" sorry (*remove old quantifier *)
+also have "... = `R1(\<exists> tr\<acute>\<acute>\<acute>\<acute> . (P[\<langle>\<rangle>/tr][($tr\<acute> - $tr)/tr\<acute>][$tr\<acute>\<acute>\<acute>\<acute>/tr\<acute>];(Q[\<langle>\<rangle>/tr][($tr\<acute> - $tr)/tr\<acute>][$tr\<acute>\<acute>\<acute>\<acute>/tr\<acute>] \<and>  ($tr \<le> $tr\<acute>\<acute>\<acute>\<acute>) \<and> ($tr\<acute>\<acute>\<acute>\<acute> \<le> $tr\<acute>))))`" sorry (*resolving substitutions *)
+also have "... = `R1(\<exists> tr\<acute>\<acute>\<acute>\<acute> . ((P[\<langle>\<rangle>/tr][($tr\<acute> - $tr)/tr\<acute>][$tr\<acute>\<acute>\<acute>\<acute>/tr\<acute>] \<and> ($tr \<le> $tr\<acute>)[$tr\<acute>\<acute>\<acute>\<acute>/tr\<acute>]);(Q[\<langle>\<rangle>/tr][($tr\<acute> - $tr)/tr\<acute>][$tr\<acute>\<acute>\<acute>\<acute>/tr] \<and> ($tr \<le> $tr\<acute>)[$tr\<acute>\<acute>\<acute>\<acute>/tr])))`" sorry (*resolving substitutions *)
+also have "... = `R1(\<exists> tr\<acute>\<acute>\<acute>\<acute> . ((P[\<langle>\<rangle>/tr][($tr\<acute> - $tr)/tr\<acute>] \<and> ($tr \<le> $tr\<acute>))[$tr\<acute>\<acute>\<acute>\<acute>/tr\<acute>];(Q[\<langle>\<rangle>/tr][($tr\<acute> - $tr)/tr\<acute>] \<and> ($tr \<le> $tr\<acute>))[$tr\<acute>\<acute>\<acute>\<acute>/tr]))`" 
+  by(simp add:usubst)
+also have "... = `R1(\<exists> tr\<acute>\<acute>\<acute> . ((P[\<langle>\<rangle>/tr][($tr\<acute> - $tr)/tr\<acute>] \<and> ($tr \<le> $tr\<acute>))[$tr\<acute>\<acute>\<acute>/tr\<acute>];(Q[\<langle>\<rangle>/tr][($tr\<acute> - $tr)/tr\<acute>] \<and> ($tr \<le> $tr\<acute>))[$tr\<acute>\<acute>\<acute>/tr]))`" sorry (*rename quantifier*)
+also have "... = `R1(\<exists> tr\<acute>\<acute>\<acute> . (R2(P)[$tr\<acute>\<acute>\<acute>/tr\<acute>];R2(Q)[$tr\<acute>\<acute>\<acute>/tr]))`" 
+  by(simp add:R1_def R2_def R2s_def)
+also have "... = `R1(R2(P);R2(Q))`"
+  apply(subst SemiR_extract_variable[where x="tr \<down>"]) back
+  apply (metis R2_rel_closure assms(1))
+  apply (metis R2_rel_closure assms(2))
+  apply (metis MkPlain_UNDASHED PVAR_VAR_MkPVAR)
+  apply (simp add:closure typing defined erasure)
+  done
+also have "... = `R2(P);R2(Q)`"
+  proof -
+  have "`R2(P);R2(Q)` is R1" 
+    by(subst R1_SemiR_closure, simp_all add: assms R2_rel_closure, simp_all add:R2_def is_healthy_def R1_idempotent)
+  thus ?thesis 
+    by (metis Healthy_simp)
+  qed
+finally show ?thesis by simp 
+qed
+
+lemma R2_composition: 
+  assumes "P \<in> WF_RELATION" "Q \<in> WF_RELATION"
+  shows "R2(P ; R2(Q)) = R2(P) ; R2(Q)"
+by (metis R2_sequential_composition assms(1) assms(2))
+    
+(* L8 R2-sequence-closure *)
+
+lemma R2_SemiR_closure: 
+assumes "P is R2" "Q is R2" "P \<in> WF_RELATION" "Q \<in> WF_RELATION"
+shows "`P;Q` is R2"
+proof -
+  have "`R2(P;Q)`=`R2(P;R2(Q))`"
+    by(metis assms(2) is_healthy_def)
+  also have "... = R2(P);R2(Q)"
+    by(metis R2_composition assms(3) assms(4))
+  also have "... = P ; Q"
+    by(metis assms is_healthy_def)
+  finally show ?thesis 
+    by (simp add:is_healthy_def)
+qed
+
+(* L10 R2-wait-okay' *)
+
+lemma R2_wait_true: "(R2(P))\<^sub>t = R2(P\<^sub>t)"
+  apply(simp add:R2_def R1_wait_true R2s_def)
+  apply(subst SubstP_twice_3) back
+  apply(simp_all)
+  apply(utp_pred_auto_tac)
+  apply(utp_pred_auto_tac)
+  apply(simp_all add:usubst typing defined closure)
+  apply(simp add:unrest closure typing defined)
+  apply(subst SubstP_twice_3) back back
+  apply(simp_all)
+  apply(utp_pred_auto_tac)
+  apply(utp_pred_auto_tac)
+  apply(simp_all add:usubst typing defined closure)
+  apply(simp add:unrest closure typing defined)
+  done
+
+lemma R2_wait_false: "(R2(P))\<^sub>f = R2(P\<^sub>f)"
+  apply(simp add:R2_def R1_wait_false R2s_def)
+  apply(subst SubstP_twice_3) back
+  apply(simp_all)
+  apply(utp_pred_auto_tac)
+  apply(utp_pred_auto_tac)
+  apply(simp_all add:usubst typing defined closure)
+  apply(simp add:unrest closure typing defined)
+  apply(subst SubstP_twice_3) back back
+  apply(simp_all)
+  apply(utp_pred_auto_tac)
+  apply(utp_pred_auto_tac)
+  apply(simp_all add:usubst typing defined closure)
+  apply(simp add:unrest closure typing defined)
+  done
+
+lemma R2_okay'_true: "(R2(P))\<^sup>t = R2(P\<^sup>t)"  
+  apply(simp add:R2_def R1_okay'_false R2s_def)
+  apply(subst SubstP_twice_3) back
+  apply(simp_all)
+  apply(utp_pred_auto_tac)
+  apply(utp_pred_auto_tac)
+  apply(simp_all add:usubst typing defined closure)
+  apply(simp add:unrest closure typing defined)
+  apply(subst SubstP_twice_3) back back
+  apply(simp_all)
+  apply(utp_pred_auto_tac)
+  apply(utp_pred_auto_tac)
+  apply(simp_all add:usubst typing defined closure)
+  apply(simp add:unrest closure typing defined)
+  apply (metis (hide_lams, no_types) PVAR_VAR_pvdash R1_okay'_true)
+  done
+
+lemma R2_okay'_false: "(R2(P))\<^sup>f = R2(P\<^sup>f)"
+  apply(simp add:R2_def R1_okay'_false R2s_def)
+  apply(subst SubstP_twice_3) back
+  apply(simp_all)
+  apply(utp_pred_auto_tac)
+  apply(utp_pred_auto_tac)
+  apply(simp_all add:usubst typing defined closure)
+  apply(simp add:unrest closure typing defined)
+  apply(subst SubstP_twice_3) back back
+  apply(simp_all)
+  apply(utp_pred_auto_tac)
+  apply(utp_pred_auto_tac)
+  apply(simp_all add:usubst typing defined closure)
+  apply(simp add:unrest closure typing defined)
+  apply (metis (hide_lams, no_types) PVAR_VAR_pvdash R1_okay'_false)
+  done
+
+(* L11 J-R2 *)
+
+lemma J_is_R2: 
+  "J is R2"
+
+proof -
+  have "R2 J = `R1 ((ok \<Rightarrow> ok') \<and> (($tr\<acute> - $tr) = \<langle>\<rangle>) \<and> II\<^bsub>REL_VAR - {okay\<down>, okay\<down>\<acute>} - {tr\<down>, tr\<down>\<acute>}\<^esub>)`"
+    apply (simp add:J_pred_def)
+    apply (subst SkipRA_unfold[of "tr \<down>"])
+    apply (simp_all)
+    apply (metis MkPlain_UNDASHED PVAR_VAR_MkPVAR)
+    apply (metis MkPlain_UNDASHED PVAR_VAR_MkPVAR UNDASHED_dash_DASHED)
+    apply (metis MkPlain_UNDASHED PVAR_VAR_MkPVAR)
+    apply (utp_pred_auto_tac)
+    apply (simp add:is_healthy_def R2_def R2s_def)
+    apply (simp add:usubst typing defined closure)
+    done
+  also have "... = `(ok \<Rightarrow> ok') \<and> R1(($tr\<acute> - $tr) = \<langle>\<rangle>) \<and> II\<^bsub>REL_VAR - {okay\<down>, okay\<down>\<acute>} - {tr\<down>, tr\<down>\<acute>}\<^esub>`"
+    by (utp_pred_auto_tac)
+  also have "... = `(ok \<Rightarrow> ok') \<and> ($tr\<acute> = $tr) \<and> II\<^bsub>REL_VAR - {okay\<down>, okay\<down>\<acute>} - {tr\<down>, tr\<down>\<acute>}\<^esub>`"
+    by (simp add:R1_def tr_prefix_as_nil)
+  also have "... = J"
+    apply(simp add:J_pred_def)
+    apply(subst SkipRA_unfold[of "tr \<down>"]) back
+    apply(simp_all)
+    apply (metis MkPlain_UNDASHED PVAR_VAR_MkPVAR)
+    apply (metis MkPlain_UNDASHED PVAR_VAR_MkPVAR UNDASHED_dash_DASHED)
+    apply (metis MkPlain_UNDASHED PVAR_VAR_MkPVAR)
+    apply (utp_pred_auto_tac)
+    apply(simp add:closure typing defined erasure)
+    done
+  finally show ?thesis 
+    by (simp add:is_healthy_def)
+qed
+
+(* L12 commutativity-R2-H1 *)
+(*No longer holds in original form since R2 has R1 like properties *)
+
+lemma H1_R2s_commute: "H1 (R2s P) = R2s (H1 P)"
+  by(simp add:H1_def R2s_def usubst typing defined closure)
+
+(* L13 commutativity R2-H2 *)
+
+lemma H2_R2_commute: 
+  assumes "P \<in> WF_RELATION"
+  shows "H2 (R2 P) = R2 (H2 P)" 
+proof -
+  have "H2 (R2 P) = (R2 P);(R2 J)" 
+    by(metis H2_def J_is_R2 is_healthy_def)
+  also have "... = R2 (P ; (R2 J))"
+    apply(subst R2_composition)
+    apply (metis assms)
+    apply (metis J_closure)
+    apply (simp)
+    done
+  also have "... = R2 (P ; J) " 
+    by(metis J_is_R2 is_healthy_def)
+  finally show ?thesis 
+    by(simp add:H2_def)
+qed
+
+(* L14 commutativity R2-R1 *)
+
+lemma R1_R2_commute: 
+  "R1 (R2 P) = R2 (R1 P)" 
+by (simp add:R2_def R1_idempotent R2s_destroys_R1)
+
+(* Additional lemmas *)
+
+lemma R2_monotonic: "P \<sqsubseteq> Q \<Longrightarrow> R2(P) \<sqsubseteq> R2(Q)" 
+  by utp_pred_tac
 
 lemma SkipRA_is_R2 : "`R2(II\<^bsub>REL_VAR - OKAY\<^esub>)` = `II\<^bsub>REL_VAR - OKAY\<^esub>`"
 proof -
@@ -222,25 +783,87 @@ proof -
   finally show ?thesis .
 qed
 
-lemma SkipREA_is_R1:
-  "`R1(II\<^bsub>rea\<^esub>)` = `II\<^bsub>rea\<^esub>`"
-  by (simp add:SkipREA_CondR_SkipR R1_CondR R1_SkipR R1_tr_leq_tr')
-
 lemma SkipREA_is_R2 : "`R2(II\<^bsub>rea\<^esub>)` = `II\<^bsub>rea\<^esub>`"
 proof-
   have "`R2(II\<^bsub>rea\<^esub>)` = `(\<not>ok \<and> ($tr \<le> $tr\<acute>)) \<or> (ok' \<and> R2(II\<^bsub>REL_VAR - OKAY\<^esub>))`" 
-    by (simp add: R2_def R1_def SkipREA_def R2s_def usubst typing defined closure, utp_pred_auto_tac)
+    apply (simp add: R2_def R1_def SkipREA_def R2s_def usubst typing defined closure)
+    apply(utp_pred_auto_tac)
+    done
   thus ?thesis 
     by (simp add:SkipRA_is_R2 SkipREA_def)
 qed
 
-lemma tr_conserved_is_R1 : "`R1($tr = $tr\<acute>)` = `($tr = $tr\<acute>)`" 
-  by (simp add:R1_def, utp_pred_auto_tac)
+subsection {* R3 Laws *}
 
-lemma tr_conserved_is_R2 : "`R2($tr = $tr\<acute>)` = `($tr = $tr\<acute>)`"
-  apply(simp add:R2_def R2s_def R1_def usubst typing defined closure)
-  apply (metis EqualP_sym tr_prefix_as_nil)
+(* L1 R3-wait-true *)
+
+lemma R3_wait_true: 
+  "`(R3(P))\<^sub>t` = `(II\<^bsub>rea\<^esub>)\<^sub>t` "
+by(simp add:R3_def usubst typing defined closure CondR_def)
+
+(* L2 R3-wait-false *)
+
+lemma R3_wait_false: 
+  "`(R3(P))\<^sub>f` = `P\<^sub>f` "
+by(simp add:R3_def usubst typing defined closure CondR_def)
+
+(* L3 R3-okay' *)
+
+lemma R3_okay'_true: 
+  "(R3(P))\<^sup>t = `II\<^bsub>rea\<^esub>\<^sup>t \<lhd> $wait \<rhd>(P\<^sup>t)`"
+by(simp add:R3_def usubst typing defined closure)
+
+lemma R3_okay'_false: 
+  "(R3(P))\<^sup>f = `II\<^bsub>rea\<^esub>\<^sup>f \<lhd> $wait \<rhd>(P\<^sup>f)`"
+by(simp add:R3_def usubst typing defined closure)
+
+(* L4 closure-\<and>-R3 *)
+
+lemma R3_AndP: 
+  "`R3(P \<and> Q)` = `R3(P) \<and> R3(Q)`"
+by(utp_pred_auto_tac)
+
+lemma R3_AndP_closure:
+  assumes "P is R3" "Q is R3"
+  shows "`P \<and> Q` is R3"
+by(metis is_healthy_def R3_AndP assms)
+
+(* L5 closure-\<or>-R3 *)
+
+lemma R3_OrP: 
+  "`R3(P \<or> Q)` = `R3(P) \<or> R3(Q)`"
+by(utp_pred_auto_tac)
+
+lemma R3_OrP_closure:
+  assumes "P is R3" "Q is R3"
+  shows "`P \<or> Q` is R3"
+by(metis is_healthy_def R3_OrP assms)
+  
+(* L6 closure-conditional-R3 *)
+
+lemma R3_CondR: 
+  "`R3(P  \<lhd> b \<rhd> Q)` = `R3(P) \<lhd> b \<rhd> R3(Q)`"
+by(utp_pred_auto_tac)
+
+lemma R3_CondR_closure:
+  assumes "P is R3" "Q is R3"
+  shows "`P \<lhd> b \<rhd> Q` is R3"
+by(metis is_healthy_def R3_CondR assms)
+
+(* L7 closure-sequence-R3 *)
+
+lemma R3_form : "`R3(P)` = `(\<not>ok \<and> $wait \<and> ($tr \<le> $tr\<acute>)) \<or> (ok \<and> $wait  \<and> II) \<or> (\<not>$wait \<and> P)`"
+  apply(simp add:R3_def SkipREA_CondR_SkipR CondR_def)
+  apply(utp_pred_auto_tac)
 done
+
+lemma R3_form_2 : "`R3(P)` = `(\<not>ok \<and> $wait \<and> ($tr \<le> $tr\<acute>)) \<or> (ok \<and> $wait  \<and> II) \<or> (\<not>$wait \<and> P\<^sub>f )`"
+proof -
+  have "`\<not>$wait \<and> P` = `\<not>$wait \<and> P\<^sub>f`"
+    sorry
+  thus ?thesis
+    by(simp add:R3_form)
+qed
 
 lemma R3_wait: "`R3(P) \<and> $wait` = `II\<^bsub>rea\<^esub> \<and> $wait`"
   apply (simp add:R3_def)
@@ -250,110 +873,190 @@ lemma R3_wait: "`R3(P) \<and> $wait` = `II\<^bsub>rea\<^esub> \<and> $wait`"
   apply (rule refl)
 done
 
-lemma R2s_idempotent: "`R2s(R2s(P))` = `R2s(P)`"
-  apply (simp add:R2s_def)
-  apply (subst SubstP_twice_3) back
-  apply (simp_all add:typing defined closure unrest)
-  apply (simp add:usubst typing defined closure)
-done
-
-lemma R2s_wait: "`R2s($wait)` = `$wait`" 
-  by (simp add:R2s_def usubst closure typing defined)
-
-lemma R2s_destroys_R1: "R2s (R1 P) = R2s P" 
-  by (simp add:R2s_def R1_def usubst closure typing defined)
-
-lemma R2s_distributes_through_conjunction: 
-  "`R2s(P \<and> Q)` = `R2s(P) \<and> R2s(Q)`" 
-  by (utp_pred_auto_tac)
-
-lemma R2s_CondR: 
-  "`R2s(P \<lhd> b \<rhd> Q)` = `R2s(P) \<lhd> R2s(b) \<rhd> R2s(Q)`"
-  by (utp_pred_auto_tac)
-
-lemma R2_idempotent: "`R2(R2(P))` = `R2(P)`" 
-  by (simp add:R2_def R2s_destroys_R1 R2s_idempotent)
-
-lemma R2_CondR: 
-  "`R2(P \<lhd> b \<rhd> Q)` =`R2(P) \<lhd> R2s(b) \<rhd> R2(Q)`" 
-  by (utp_pred_auto_tac)
-
-lemma R2_CondR_alt: 
-  "`R2(P \<lhd> b \<rhd> Q)` =`R2(P) \<lhd> R2(b) \<rhd> R2(Q)`" 
-  by (utp_pred_auto_tac)
-
-lemma R2s_OrP: 
-  "`R2s(A \<or> C)` = `R2s(A) \<or> R2s(C)`" 
-  by (utp_pred_auto_tac)
-
-lemma R1_not_ok: "`R1(\<not> ok)` = `(\<not> ok \<and> ($tr \<le> $tr\<acute>))`" 
-  by (simp add:R1_def)
-
-lemma R2s_not_ok: "`R2s(\<not> ok)` = `\<not> ok`" 
-  by (simp add:R2s_def usubst typing defined closure) 
-
-lemma R2_not_ok: "`R2(\<not> ok)` = `R1(\<not> ok)`"
-  by (simp add:R2_def usubst typing defined closure R2s_not_ok) 
-
-lemma R2_AndP: "`R2(P \<and> Q)` = `R2(P) \<and> R2(Q)`"
-  by (utp_pred_auto_tac)
-
-lemma R2_OrP: "`R2(P \<or> Q)` = `R2(P) \<or> R2(Q)`"
-  by (utp_pred_auto_tac)
-
-lemma R3_SkipREA: "`R3(II\<^bsub>rea\<^esub>)` = `II\<^bsub>rea\<^esub>`"
-  by (simp add:R3_def CondR_idem)
-
-lemma R3_AndP: "`R3(P \<and> Q)` = `R3(P) \<and> R3(Q)`"
-  by (utp_pred_auto_tac)
-
-lemma R3_OrP:
-  "`R3(P \<or> Q)` = `R3(P) \<or> R3(Q)`"
-  by (utp_pred_auto_tac)
-
-lemma R3_CondR:
-  "`R3(P \<lhd> b \<rhd> Q)` = `R3(P) \<lhd> R3(b) \<rhd> R3(Q)`"
-  by (utp_pred_auto_tac)
-
-(*
-theorem R3_SemiR [closure]:
+theorem R3_SemiR_closure [closure]:
   assumes
     "P \<in> WF_RELATION" "Q \<in> WF_RELATION"
-    "P is R3"
+    "P is R3" "Q is R3" "Q is R1"
   shows "(P ; Q) is R3"
 proof -
-  have "`P ; Q` = `(II\<^bsub>rea\<^esub> \<lhd> $wait \<rhd> P) ; Q`"
-    by (metis Healthy_elim R3_def assms(3))
-
-  also have "... = `(II\<^bsub>rea\<^esub> ; Q) \<lhd> $wait \<rhd> (P ; Q)`"
-    by (metis CondR_SemiR_distr MkPlainP_UNDASHED PUNDASHED_WF_CONDITION SkipREA_rel_closure assms)
-
-  also have "... = `II\<^bsub>rea\<^esub> \<lhd> $wait \<rhd> (P ; Q)`"
-
-  also have "... = `R3(P ; Q)`"
-    by (metis R3_def)
-    
-    apply (simp add:CondR_SemiR_distl closure unrest assms)
-
-    apply (simp add:R3_def)
-    by (metis Healthy_elim assms(3))
+  have "`(\<not>ok \<and> $wait \<and> ($tr \<le> $tr\<acute>));Q` = `\<not>ok \<and> $wait \<and> (($tr \<le> $tr\<acute>);Q)`"
+    apply(subst SemiR_AndP_left_precond)
+    apply (metis MkPlainP_UNDASHED PUNDASHED_WF_CONDITION R1_def R1_rel_closure WF_CONDITION_WF_RELATION)
+    apply (metis assms(2))
+    apply (metis TopD_cond_closure TopD_def)
+    apply(subst SemiR_AndP_left_precond)
+    apply (simp_all)
+    apply (metis R1_def R1_rel_closure TrueP_rel_closure utp_pred_simps(6))
+    apply (metis assms(2))
+    apply (metis MkPlainP_UNDASHED PUNDASHED_WF_CONDITION)
+    done
+  moreover have "`($tr \<le> $tr\<acute>) ; Q ` = `($tr \<le> $tr\<acute>)`"
+  proof-
+    have 1: "`(($tr \<le> $tr\<acute>) ; (\<not>ok \<and> $wait \<and> ($tr \<le> $tr\<acute>)))`=`($tr \<le> $tr\<acute>)`"
+      by (metis Aida)
+    have 2: "`(($tr \<le> $tr\<acute>);(ok \<and> $wait \<and> II))` is R1" 
+      apply(subst R1_SemiR_closure)
+      apply(simp_all)
+      apply (metis R1_def R1_rel_closure TrueP_rel_closure utp_pred_simps(6))
+      apply (metis AndP_rel_closure MkPlainP_UNDASHED PUNDASHED_WF_CONDITION SkipR_closure WF_CONDITION_WF_RELATION)
+      apply (metis R1_by_refinement order_refl)
+      apply (metis (full_types) AndP_comm Healthy_intro R1_SkipR R1_extend_AndP)
+      done
+    have 3: "`(($tr \<le> $tr\<acute>);(\<not>$wait \<and> Q))` is R1"
+      apply(subst R1_SemiR_closure)
+      apply(simp_all)
+      apply (metis R1_def R1_rel_closure TrueP_rel_closure utp_pred_simps(6))
+      apply (metis AndP_rel_closure MkPlainP_UNDASHED NotP_rel_closure PUNDASHED_WF_CONDITION WF_CONDITION_WF_RELATION assms(2))
+      apply (metis R1_by_refinement order_refl)  
+      apply (metis (full_types) AndP_comm R1_extend_AndP assms(5) is_healthy_def)
+      done
+    have "`($tr \<le> $tr\<acute>) ; Q` = `($tr \<le> $tr\<acute>) ; R3(Q)`"
+      by (metis Healthy_simp assms)
+    also have "... = `(($tr \<le> $tr\<acute>) ; (\<not>ok \<and> $wait \<and> ($tr \<le> $tr\<acute>))) \<or> (($tr \<le> $tr\<acute>);(ok \<and> $wait \<and> II)) \<or> (($tr \<le> $tr\<acute>);(\<not>$wait \<and> Q))`"
+      by(simp add:R3_form SemiR_OrP_distl)
+    also have "... = `($tr \<le> $tr\<acute>) \<or> R1(($tr \<le> $tr\<acute>);(ok \<and> $wait \<and> II)) \<or> R1(($tr \<le> $tr\<acute>);(\<not>$wait \<and> Q))`"
+      by(metis 1 2 3 is_healthy_def)
+    also have "... = `($tr \<le> $tr\<acute>)`"
+      by(utp_pred_auto_tac)
+    finally show ?thesis 
+      ..
+  qed
+  ultimately have 1: "`(\<not>ok \<and> $wait \<and> ($tr \<le> $tr\<acute>)) ; Q` = `\<not>ok \<and> $wait \<and> ($tr \<le> $tr\<acute>)`" by metis
+  have a : "`((($okay \<and> $wait \<and> II) \<and> ($okay)\<acute>) \<and> ($wait)\<acute>)` = `ok \<and> ok' \<and> $wait \<and> $wait\<acute> \<and> II`"
+    by (smt AndP_assoc AndP_comm ConvR_VarP_1 MkPlainP_UNDASHED PVAR_VAR_PUNDASHED_UNDASHED PVAR_VAR_pvdash)
+  have 2: "`(ok \<and> $wait \<and> II);Q` = `ok \<and> $wait \<and> II`"
+    proof -
+      have "`ok \<and> $wait \<and> II` = `ok \<and> $wait \<and> ($okay\<acute> = $okay) \<and> ($wait\<acute> = $wait) \<and> II`"
+        apply (simp add:SkipR_as_SkipRA)
+        apply (subst SkipRA_unfold[of "okay \<down>"])
+        apply(simp_all)
+        apply (metis MkPlainP_UNDASHED PVAR_VAR_PUNDASHED_UNDASHED)
+        apply(utp_pred_auto_tac)
+        apply (metis MkPlainP_UNDASHED PVAR_VAR_PUNDASHED_UNDASHED)
+        apply (subst SkipRA_unfold[of "okay \<down>"]) back
+        apply(simp_all)
+        apply (metis MkPlainP_UNDASHED PVAR_VAR_PUNDASHED_UNDASHED)
+        apply(utp_pred_auto_tac)
+        apply (metis MkPlainP_UNDASHED PVAR_VAR_PUNDASHED_UNDASHED)
+        apply (subst SkipRA_unfold[of "wait \<down>"])
+        apply(simp_all)
+        apply (metis MkPlainP_UNDASHED PVAR_VAR_PUNDASHED_UNDASHED)
+        apply(utp_pred_auto_tac)
+        apply (metis MkPlainP_UNDASHED PVAR_VAR_PUNDASHED_UNDASHED)
+        apply(utp_pred_auto_tac)
+        apply (subst SkipRA_unfold[of "wait \<down>"]) back
+        apply(simp_all)
+        apply (metis MkPlainP_UNDASHED PVAR_VAR_PUNDASHED_UNDASHED)
+        apply(utp_pred_auto_tac)
+        apply (metis MkPlainP_UNDASHED PVAR_VAR_PUNDASHED_UNDASHED)
+        apply(utp_pred_auto_tac)
+        apply(simp add:erasure typing defined closure)
+        apply (smt AndP_assoc AndP_idem)
+        done
+      also have "... = `ok \<and> ok' \<and> $wait \<and> $wait\<acute> \<and> II`"
+        by (smt AndP_assoc AndP_comm Aidb Aidc)
+      finally have "`(ok \<and> $wait \<and> II);R3(Q)` = `(ok \<and> ok' \<and> $wait \<and> $wait\<acute> \<and> II);R3(Q)`" 
+        by metis
+      also have "... = `(ok \<and> $wait \<and> II);(ok \<and> $wait \<and> R3(Q))`" 
+        apply(subst SemiR_AndP_right_precond)
+        apply (metis AndP_rel_closure MkPlainP_UNDASHED PUNDASHED_WF_CONDITION SkipR_closure WF_CONDITION_WF_RELATION)
+        apply (metis AndP_rel_closure MkPlainP_UNDASHED PUNDASHED_WF_CONDITION WF_CONDITION_WF_RELATION assms(2) assms(4) is_healthy_def)
+        apply (metis MkPlainP_UNDASHED PUNDASHED_WF_CONDITION)
+        apply(subst SemiR_AndP_right_precond)
+        apply (smt AndP_rel_closure ConvR_rel_closure MkPlainP_UNDASHED PUNDASHED_WF_CONDITION SkipR_closure WF_CONDITION_WF_RELATION)
+        apply (metis R3_rel_closure assms(2))
+        apply (metis MkPlainP_UNDASHED PUNDASHED_WF_CONDITION)
+        apply (metis a)
+        done
+      also have "... = `(ok \<and> $wait \<and> II);(ok \<and> $wait \<and> II)`"
+        proof -
+          have "`ok \<and> $wait \<and> R3(Q)` = `ok \<and> $wait \<and> II`" 
+            apply(simp add:R3_form) 
+            apply(utp_pred_auto_tac) 
+            done
+          thus ?thesis 
+            by metis
+        qed
+      also have "... = `(ok \<and> ok' \<and> $wait \<and> $wait\<acute> \<and> II);II`"
+        apply(subst SemiR_AndP_right_precond)
+        apply (metis AndP_rel_closure MkPlainP_UNDASHED PUNDASHED_WF_CONDITION SkipR_closure WF_CONDITION_WF_RELATION)
+        apply (metis (full_types) AndP_rel_closure MkPlainP_UNDASHED PUNDASHED_WF_CONDITION SkipR_closure WF_CONDITION_WF_RELATION)
+        apply (metis MkPlainP_UNDASHED PUNDASHED_WF_CONDITION)
+        apply(subst SemiR_AndP_right_precond)
+        apply (smt AndP_rel_closure ConvR_rel_closure MkPlainP_UNDASHED PUNDASHED_WF_CONDITION SkipR_closure WF_CONDITION_WF_RELATION)
+        apply (metis SkipR_closure)
+        apply (metis MkPlainP_UNDASHED PUNDASHED_WF_CONDITION)
+        apply (metis a)
+        done
+      also have "... = `ok \<and> ok' \<and> $wait \<and> $wait\<acute> \<and> II`"by (metis SemiR_SkipR_right)
+      also have "... = `ok \<and> $wait \<and> II`"
+      proof -
+        have "`ok \<and> ok' \<and> $wait \<and> $wait\<acute> \<and> II` =  `ok \<and> $wait \<and> ($okay\<acute> = $okay) \<and> ($wait\<acute> = $wait) \<and> II`"
+          by (smt AndP_assoc AndP_comm Aidb Aidc)
+        also have "... = `ok \<and> $wait \<and> II`"
+          apply (simp add:SkipR_as_SkipRA)
+          apply (subst SkipRA_unfold[of "okay \<down>"])
+          apply(simp_all)
+          apply (metis MkPlainP_UNDASHED PVAR_VAR_PUNDASHED_UNDASHED)
+          apply(utp_pred_auto_tac)
+          apply (metis MkPlainP_UNDASHED PVAR_VAR_PUNDASHED_UNDASHED)
+          apply (subst SkipRA_unfold[of "okay \<down>"]) back
+          apply(simp_all)
+          apply (metis MkPlainP_UNDASHED PVAR_VAR_PUNDASHED_UNDASHED)
+          apply(utp_pred_auto_tac)
+          apply (metis MkPlainP_UNDASHED PVAR_VAR_PUNDASHED_UNDASHED)
+          apply (subst SkipRA_unfold[of "wait \<down>"])
+          apply(simp_all)
+          apply (metis MkPlainP_UNDASHED PVAR_VAR_PUNDASHED_UNDASHED)
+          apply(utp_pred_auto_tac)
+          apply (metis MkPlainP_UNDASHED PVAR_VAR_PUNDASHED_UNDASHED)
+          apply(utp_pred_auto_tac)
+          apply (subst SkipRA_unfold[of "wait \<down>"]) back
+          apply(simp_all)
+          apply (metis MkPlainP_UNDASHED PVAR_VAR_PUNDASHED_UNDASHED)
+          apply(utp_pred_auto_tac)
+          apply (metis MkPlainP_UNDASHED PVAR_VAR_PUNDASHED_UNDASHED)
+          apply(utp_pred_auto_tac)
+          apply(simp add:erasure typing defined closure)
+          apply (smt AndP_assoc AndP_idem)
+          done
+        finally show ?thesis
+          ..
+      qed
+      finally show ?thesis 
+        by (metis assms(4) is_healthy_def)
+    qed
+  have 3: "`(\<not> $wait \<and> P);Q` = `\<not> $wait \<and> (P;Q)`"
+    by(subst SemiR_AndP_left_precond, simp_all add:assms, utp_pred_auto_tac)
+  have "`P ; Q` = `R3(P) ; Q`" 
+    by (metis assms(3) is_healthy_def)
+  also have "... = `(\<not>ok \<and> $wait \<and> ($tr \<le> $tr\<acute>));Q  \<or> (ok \<and> $wait \<and> II);Q \<or> (\<not> $wait \<and> P);Q`" 
+    by(simp add:R3_form SemiR_OrP_distr)
+  also have "... = `(\<not>ok \<and> $wait \<and> ($tr \<le> $tr\<acute>))  \<or> (ok \<and> $wait \<and> II) \<or> (\<not> $wait \<and> (P;Q))`"
+    by (metis "1" "2" "3") 
+  finally show ?thesis 
+    by (simp add:R3_form is_healthy_def)
 qed
-*)
+
+(* L8 R3-idempotent *)
 
 lemma R3_idempotent: "`R3(R3(P))` = `R3(P)`" 
   by (utp_pred_auto_tac)
 
-lemma R1_monotonic: "P \<sqsubseteq> Q \<Longrightarrow> R1(P) \<sqsubseteq> R1(Q)" 
-  by utp_pred_tac
+(* L9 commutativity-R3-H2 *)
 
-lemma R2_monotonic: "P \<sqsubseteq> Q \<Longrightarrow> R2(P) \<sqsubseteq> R2(Q)" 
-  by utp_pred_tac
+lemma H2_R3_commute: 
+  assumes "P \<in> WF_RELATION"
+  shows "H2 (R3 P) = R3 (H2 P)" 
+  apply(simp add:R3_def CondR_def H2_def SemiR_OrP_distr)
+  apply(subst SemiR_AndP_left_precond[of _ _ "`$wait`"])
+  apply(simp_all add:SkipREA_rel_closure J_closure MkPlainP_UNDASHED PUNDASHED_WF_CONDITION)
+  apply(subst SemiR_AndP_left_precond[of _ _ "`\<not>$wait`"])
+  apply(simp_all add:assms J_closure MkPlainP_UNDASHED NotP_cond_closure PUNDASHED_WF_CONDITION) 
+  apply (metis H2_SkipREA H2_def)
+  done
 
-lemma R3_monotonic: "P \<sqsubseteq> Q \<Longrightarrow> R3(P) \<sqsubseteq> R3(Q)" 
-  by utp_pred_tac
-
-lemma R1_R2_commute: "R1 (R2 P) = R2 (R1 P)" 
-  by (simp add:R2_def R1_idempotent R2s_destroys_R1)
+(* L10 commutativity-R3-R1 *)
 
 lemma R1_R3_commute: "R1 (R3 P) = R3 (R1 P)" 
 proof - 
@@ -366,19 +1069,52 @@ proof -
   ultimately show ?thesis by utp_pred_auto_tac
 qed
 
+(* L11 commutativite-R3-R2 *)
+
 theorem R2_R3_commute: 
   "R2 (R3 P) = R3 (R2 P)" 
 proof - 
   have "R2 (R3 P) = `R2(II\<^bsub>rea\<^esub>) \<lhd> R2s($wait) \<rhd> R2(P)`" 
     by (simp add:R3_def R2_CondR)
-  also have "... = `II\<^bsub>rea\<^esub> \<lhd> $wait \<rhd> R2(P)`" 
-    by (simp add: SkipREA_is_R2 R2s_wait)
+  also have "... = `II\<^bsub>rea\<^esub> \<lhd> $wait \<rhd> R2(P)`"
+    by (simp add: SkipREA_is_R2 R2s_def usubst typing defined closure)
   finally show ?thesis 
     by (simp add: R3_def R2_def)
 qed
 
-lemma helper1 : "`$wait \<and> II\<^bsub>REL_VAR - {okay\<down>, okay\<down>\<acute>}\<^esub>` = `$wait \<and> $wait\<acute> \<and> II\<^bsub>REL_VAR - {okay\<down>, okay\<down>\<acute>}\<^esub>`"
-  by (auto simp add:var_dist closure evalr evale)
+(* L12 R3-H1-sub-commutativity *)
+
+lemma R3_H1_sub_commute: 
+  "H1 (R3 P) = H1 (R3 (H1 P))"
+by(utp_pred_auto_tac)
+
+(* L13 R3-H1-R1-sub-commutativity *)
+
+lemma R3_H1_R1_sub_commute: 
+  "R3 (R1 (H1 P)) = R1 (H1 (R3 P))"
+proof -
+  have "R3 (R1 (H1 P)) = `($wait \<and> II\<^bsub>rea\<^esub>) \<or> (\<not>$wait \<and> ($tr\<le>$tr\<acute>) \<and> \<not>ok) \<or> (\<not>$wait \<and> ($tr\<le>$tr\<acute>) \<and> P)`" 
+    by utp_pred_auto_tac
+  also have "... = `($wait \<and> II\<^bsub>rea\<^esub> \<and> ($tr\<le>$tr\<acute>)) \<or> (\<not>$wait \<and> ($tr\<le>$tr\<acute>) \<and> \<not>ok) \<or> (\<not>$wait \<and> ($tr\<le>$tr\<acute>) \<and> P)`"
+    proof -
+      have "`II\<^bsub>rea\<^esub>` = `II\<^bsub>rea\<^esub> \<and> ($tr\<le>$tr\<acute>)` "
+        by (metis R1_def SkipREA_is_R1)
+      thus ?thesis 
+        by metis
+    qed
+  finally show ?thesis 
+    by utp_pred_auto_tac
+qed
+
+(* Additional Lemmas *)
+
+lemma R3_SkipREA: "`R3(II\<^bsub>rea\<^esub>)` = `II\<^bsub>rea\<^esub>`"
+  by (simp add:R3_def CondR_idem)
+
+lemma R3_monotonic: "P \<sqsubseteq> Q \<Longrightarrow> R3(P) \<sqsubseteq> R3(Q)" 
+  by utp_pred_tac
+
+subsection {* RH Laws *}
 
 lemma RH_is_R1:
   "P is RH \<Longrightarrow> P is R1"
@@ -395,36 +1131,210 @@ lemma RH_is_R3:
 lemma R_intro: "\<lbrakk> P is R1; P is R2; P is R3 \<rbrakk> \<Longrightarrow> P is RH"
   by (metis RH_def comp_apply is_healthy_def)
 
-(*
-lemma helper2: "`($wait\<acute> \<and> Q) ; R3(P)` = `$wait\<acute> \<and> Q`" sorry
-lemma helper4 : "`\<langle>\<rangle> = ($tr\<acute> - $tr)` =`$tr\<acute> = $tr`" sorry
-lemma wait_then_P_equals_wait : "`(($wait \<and> II\<^bsub>rea\<^esub>) \<and> ($tr \<le> $tr\<acute>)) ; P` = `(($wait \<and> II\<^bsub>rea\<^esub>) \<and> ($tr \<le> $tr\<acute>))`" sorry
-lemma R2s_R3_commute : "R2s (R3 P) = R3 (R2s P)" sorry
-lemma Assist : "`P[false/okay\<acute>] \<or> P[true/okay\<acute>]` = `P`"sorry
-lemma Assist7 : "`(($tr < $tr\<acute>) \<and> ($tr^\<langle>a\<rangle> =$tr\<acute>))` = `($tr^\<langle>a\<rangle> =$tr\<acute>)`" sorry
+(* L1 reactive-left-zero *)
 
-lemma conj_distributes_through_conditional : "`(P \<lhd> b \<rhd> Q) \<and> S` = `(P \<and> S)\<lhd> b \<rhd>(Q \<and> S)`"by utp_pred_auto_tac
-lemma R2s_distributes_through_conjunction : "`R2s(P \<and> Q)` = `R2s(P) \<and> R2s(Q)`" by utp_pred_auto_tac
-lemma R2s_distributes_through_conditional : "`R2s(P \<lhd> b \<rhd> Q)` = `R2s(P)\<lhd> R2s(b) \<rhd>R2s(Q)`"by utp_pred_auto_tac
-lemma R3_distributes_through_disjunction :"`R3(P \<or> Q)` = `R3(P) \<or> R3(Q)`"by utp_pred_auto_tac
-lemma R3_distributes_through_conditional :"`R3(P \<lhd> b \<rhd> Q)` = `R3(P) \<lhd> R3(b) \<rhd> R3(Q)`"by utp_pred_auto_tac
-lemma seq_comp_assoc : "`(P ; Q) ; S` = `P ; (Q ; S)`"by (metis SemiR_assoc)
-lemma R2s_distributes_through_disjunction: "`R2s(A \<or> C)` = `R2s(A) \<or> R2s(C)`" by utp_pred_auto_tac
-lemma R1_not_ok : "`(\<not> ok \<and> ($tr \<le> $tr\<acute>))` = `R1(\<not> ok)`" by (simp add:R1_def)
-lemma not_ok_is_R2s : "`R2s(\<not> ok)` = `\<not> ok`" by (simp add:R2s_def usubst typing defined closure) 
-lemma ok_dash_is_R2s : "`R2s(ok')` = `ok'`"by (simp add:R2s_def usubst typing defined closure)
-lemma Assist5 : "`R1(P \<and> Q)` = `P \<and> R1(Q)`" by utp_pred_auto_tac
-lemma wait_is_R2 : "`$wait[($tr\<acute> - $tr)/tr\<acute>][\<langle>\<rangle>/tr]` = `$wait`" by(simp add:usubst typing defined closure)
-lemma not_wait_is_R2 : "`(\<not> $wait)[($tr\<acute> - $tr)/tr\<acute>][\<langle>\<rangle>/tr]` = `\<not> $wait`" by(simp add:usubst typing defined closure)
-lemma conj_through_dist_2 : "`P \<and> Q \<or> S` = `(P \<and> Q) \<or> (P \<and> S)`" by utp_pred_auto_tac
-lemma negation_of_disjunction  : "`\<not>(P \<or> Q)` = `(\<not>P \<and> \<not>Q)`" by utp_pred_auto_tac
-lemma aider3 : "`$okay\<acute> \<and> II\<^bsub>rea\<^esub>[true/okay\<acute>]` = `$okay\<acute> \<and> II\<^bsub>rea\<^esub>`"by(simp add:SkipREA_def usubst typing defined closure, utp_pred_auto_tac)
-*)
+lemma R1_true_left_zero: 
+  assumes "P is R1" "P is R3" "P \<in> WF_RELATION"
+  shows "`($tr \<le> $tr\<acute>) ; P` = `($tr \<le> $tr\<acute>)`"
+proof -
+  have 1: "`(($tr \<le> $tr\<acute>) ; (\<not>ok \<and> $wait \<and> ($tr \<le> $tr\<acute>)))`=`($tr \<le> $tr\<acute>)`"
+    by (metis Aida)
+  have 2: "`(($tr \<le> $tr\<acute>);(ok \<and> $wait \<and> II))` is R1" 
+    apply(subst R1_SemiR_closure)
+    apply(simp_all)
+    apply (metis R1_def R1_rel_closure TrueP_rel_closure utp_pred_simps(6))
+    apply (metis AndP_rel_closure MkPlainP_UNDASHED PUNDASHED_WF_CONDITION SkipR_closure WF_CONDITION_WF_RELATION)
+    apply (metis R1_by_refinement order_refl)
+    apply (metis (full_types) AndP_comm Healthy_intro R1_SkipR R1_extend_AndP)
+    done
+  have 3: "`(($tr \<le> $tr\<acute>);(\<not>$wait \<and> P))` is R1"
+    apply(subst R1_SemiR_closure)
+    apply(simp_all)
+    apply (metis R1_def R1_rel_closure TrueP_rel_closure utp_pred_simps(6))
+    apply (metis AndP_rel_closure MkPlainP_UNDASHED NotP_rel_closure PUNDASHED_WF_CONDITION WF_CONDITION_WF_RELATION assms(3))
+    apply (metis R1_by_refinement order_refl)  
+    apply (metis (full_types) AndP_comm R1_extend_AndP RH_is_R1 assms(1) is_healthy_def)
+    done
+  have "`($tr \<le> $tr\<acute>) ; P` = `($tr \<le> $tr\<acute>) ; R3(P)`"
+    by (metis Healthy_simp RH_is_R3 assms)
+  also have "... = `(($tr \<le> $tr\<acute>) ; (\<not>ok \<and> $wait \<and> ($tr \<le> $tr\<acute>))) \<or> (($tr \<le> $tr\<acute>);(ok \<and> $wait \<and> II)) \<or> (($tr \<le> $tr\<acute>);(\<not>$wait \<and> P))`"
+    by(simp add:R3_form SemiR_OrP_distl)
+  also have "... = `($tr \<le> $tr\<acute>) \<or> R1(($tr \<le> $tr\<acute>);(ok \<and> $wait \<and> II)) \<or> R1(($tr \<le> $tr\<acute>);(\<not>$wait \<and> P))`"
+    by(metis 1 2 3 is_healthy_def)
+  also have "... = `($tr \<le> $tr\<acute>)`"
+    by(utp_pred_auto_tac)
+  finally show ?thesis 
+    ..
+qed
+
+(* L2 restricted-identity *)
+
+lemma SkipREA_restricted_identity:
+  assumes "P is RH" "P \<in> WF_RELATION"
+  shows " `II\<^bsub>rea\<^esub>; P` = `P \<lhd> ok \<rhd> ($tr \<le> $tr\<acute>)`"
+  apply (simp add:SkipREA_CondR_SkipR CondR_def SemiR_OrP_distr)
+  apply (subst SemiR_AndP_left_precond[of _ _ "`ok`"])
+  apply (simp_all add:SkipR_closure assms(2) MkPlainP_UNDASHED PUNDASHED_WF_CONDITION)
+  apply (subst SemiR_AndP_left_precond[of _ _ "`\<not>ok`"])
+  apply (simp_all add:assms(2))
+  apply (metis R1_def R1_rel_closure TrueP_rel_closure utp_pred_simps(6))
+  apply (metis TopD_cond_closure TopD_def)
+  apply (subst R1_true_left_zero)
+  apply (simp_all add:assms)
+  apply (metis RH_is_R1 assms(1))
+  apply (metis RH_is_R3 assms(1))
+  done
+
+(* L3 R-wait-false *)
+
+lemma RH_wait_false: 
+  "`(RH(P))\<^sub>f` = `R1(R2(P\<^sub>f))`"
+by(simp add:RH_def R1_wait_false R2_wait_false R3_wait_false)
+
+(* L4 R-wait-true *)
+
+lemma RH_wait_true: 
+  "`(RH(P))\<^sub>t` = `II\<^bsub>rea\<^esub>\<^sub>t`"
+proof -
+  have 1: "`II\<^bsub>rea\<^esub>\<^sub>t` = `(\<not>ok \<and> ($tr \<le> $tr\<acute>)) \<or> (ok' \<and> $wait\<acute> \<and> II\<^bsub>REL_VAR - {okay\<down>, okay\<down>\<acute>} - {wait\<down>, wait\<down>\<acute>}\<^esub>)`"
+    apply(simp add:SkipREA_def usubst typing defined closure)
+    apply (metis (hide_lams, no_types) Aidd PVAR_VAR_pvdash)
+    done
+  have "`(RH(P))\<^sub>t` = R1 (R2 `II\<^bsub>rea\<^esub>\<^sub>t`)"
+    by(simp add: RH_def R1_wait_true R2_wait_true R3_wait_true)
+  also from 1 have "... = R1 (R2 `(\<not>ok \<and> ($tr \<le> $tr\<acute>)) \<or> (ok' \<and> $wait\<acute> \<and> II\<^bsub>REL_VAR - {okay\<down>, okay\<down>\<acute>} - {wait\<down>, wait\<down>\<acute>}\<^esub>)`)"
+    by(metis)
+  also have "... = `R1 (\<not>ok) \<or> R1 (ok' \<and> $wait\<acute> \<and> (($tr\<acute> - $tr) = \<langle>\<rangle>) \<and> II\<^bsub>REL_VAR - {okay\<down>, okay\<down>\<acute>} - {wait\<down>, wait\<down>\<acute>} - {tr\<down>, tr\<down>\<acute>}\<^esub>)`" 
+    apply(simp add: R2_def R1_idempotent)
+    apply(subst SkipRA_unfold[of "tr \<down>"])
+    apply(simp_all)
+    apply (metis MkPlain_UNDASHED PVAR_VAR_MkPVAR)
+    apply (metis MkPlain_UNDASHED PVAR_VAR_MkPVAR UNDASHED_dash_DASHED)
+    apply (metis MkPlain_UNDASHED PVAR_VAR_MkPVAR)
+    apply (smt HOMOGENEOUS_REL_VAR HOMOGENEOUS_empty HOMOGENEOUS_insert HOMOGENEOUS_minus MkPlainP_UNDASHED PVAR_VAR_PUNDASHED_UNDASHED)
+    apply(simp add:R2s_def usubst typing defined closure R1_OrP)
+    done
+  also have "... = `(\<not>ok \<and> ($tr \<le> $tr\<acute>)) \<or> (ok' \<and> $wait\<acute> \<and> R1(($tr\<acute> - $tr) = \<langle>\<rangle>) \<and> II\<^bsub>REL_VAR - {okay\<down>, okay\<down>\<acute>} - {wait\<down>, wait\<down>\<acute>} - {tr\<down>, tr\<down>\<acute>}\<^esub>)`"
+    by(utp_pred_auto_tac)
+  also have "... = `(\<not>ok \<and> ($tr \<le> $tr\<acute>)) \<or> (ok' \<and> $wait\<acute> \<and> ($tr\<acute> = $tr) \<and> II\<^bsub>REL_VAR - {okay\<down>, okay\<down>\<acute>} - {wait\<down>, wait\<down>\<acute>} - {tr\<down>, tr\<down>\<acute>}\<^esub>)`"
+    by (smt R1_def tr_prefix_as_nil)
+  also have "... = `(\<not>ok \<and> ($tr \<le> $tr\<acute>)) \<or> (ok' \<and> $wait\<acute> \<and> II\<^bsub>REL_VAR - {okay\<down>, okay\<down>\<acute>} - {wait\<down>, wait\<down>\<acute>}\<^esub>)`"
+    apply(subst SkipRA_unfold[of "tr \<down>"]) back
+    apply(simp_all)
+    apply (metis MkPlain_UNDASHED PVAR_VAR_MkPVAR)
+    apply (metis MkPlain_UNDASHED PVAR_VAR_MkPVAR UNDASHED_dash_DASHED)
+    apply (metis MkPlain_UNDASHED PVAR_VAR_MkPVAR)
+    apply (smt HOMOGENEOUS_REL_VAR HOMOGENEOUS_empty HOMOGENEOUS_insert HOMOGENEOUS_minus MkPlainP_UNDASHED PVAR_VAR_PUNDASHED_UNDASHED)
+    apply(simp add:erasure typing closure defined)
+    done
+  also from 1 have "... = `II\<^bsub>rea\<^esub>\<^sub>t`" 
+    by metis
+  finally show ?thesis
+    ..
+qed
+
+(* L5 R-okay' *)
+
+lemma RH_okay'_true: 
+  "(RH(P))\<^sup>t = `II\<^bsub>rea\<^esub>\<^sup>t \<lhd> $wait \<rhd>R1(R2(P\<^sup>t))`"
+proof-
+  have "(R1(R2(P)))\<^sup>t = R1(R2(P\<^sup>t))" 
+    by (metis R1_okay'_true R2_okay'_true)
+  hence "(R3(R1(R2(P))))\<^sup>t = `II\<^bsub>rea\<^esub>\<^sup>t \<lhd> $wait \<rhd>R1(R2(P\<^sup>t))`" 
+    by (smt R3_okay'_true)
+  thus ?thesis 
+    by(simp add:RH_def R2_R3_commute R1_R3_commute)
+qed
+
+lemma RH_okay'_false: 
+  "(RH(P))\<^sup>f = `II\<^bsub>rea\<^esub>\<^sup>f \<lhd> $wait \<rhd>R1(R2(P\<^sup>f))`"
+proof-
+  have "(R1(R2(P)))\<^sup>f = R1(R2(P\<^sup>f))" 
+    by (metis R1_okay'_false R2_okay'_false)
+  hence "(R3(R1(R2(P))))\<^sup>f = `II\<^bsub>rea\<^esub>\<^sup>f \<lhd> $wait \<rhd>R1(R2(P\<^sup>f))`" 
+    by (smt R3_okay'_false)
+  thus ?thesis 
+    by(simp add:RH_def R2_R3_commute R1_R3_commute)
+qed
+
+(* L6 closure-\<and>-R *)
+
+lemma RH_AndP_closure:
+  assumes "P is RH" "Q is RH"
+  shows "`P \<and> Q` is RH"
+proof -
+  have "`R3(P \<and> Q)` = `P \<and> Q`" 
+    by (metis Healthy_simp R3_AndP RH_is_R3 assms(1) assms(2))
+  hence "`R2(R3(P \<and> Q))` = `P \<and> Q`" 
+    by (metis R2_AndP RH_is_R2 assms(1) assms(2) is_healthy_def)
+  hence "`R1(R2(R3(P \<and> Q)))` = `P \<and> Q`" 
+    by (metis R1_idempotent R2_def)
+  thus ?thesis 
+    by(simp add:is_healthy_def RH_def)
+qed
+
+(* L7 closure-\<or>-R *)
+
+lemma RH_OrP_closure:
+  assumes "P is RH" "Q is RH"
+  shows "`P \<or> Q` is RH"
+proof -
+  have "`R3(P \<or> Q)` = `P \<or> Q`" 
+    by (metis Healthy_simp R3_OrP RH_is_R3 assms(1) assms(2))
+  hence "`R2(R3(P \<or> Q))` = `P \<or> Q`" 
+    by (metis R2_OrP RH_is_R2 assms(1) assms(2) is_healthy_def)
+  hence "`R1(R2(R3(P \<or> Q)))` = `P \<or> Q`" 
+    by (metis R1_idempotent R2_def)
+  thus ?thesis 
+    by(simp add:is_healthy_def RH_def)
+qed
+
+(* L8 closure-cond-R *)
+
+lemma RH_CondR_closure:
+  assumes "P is RH" "Q is RH" "b is R2s"
+  shows "`P \<lhd> b \<rhd> Q` is RH"
+proof -
+  have "`R3(P \<lhd> b \<rhd> Q)` = `P \<lhd> b \<rhd> Q`" by (metis Healthy_simp R3_CondR RH_is_R3 assms(1) assms(2))
+  hence "`R2(R3(P \<lhd> b \<rhd> Q))` = `P \<lhd> b \<rhd> Q`" by (metis R2_CondR RH_is_R2 assms(1) assms(2) assms(3) is_healthy_def)
+  hence "`R1(R2(R3(P \<lhd> b \<rhd> Q)))` = `P \<lhd> b \<rhd> Q`" by (metis R1_idempotent R2_def)
+  thus ?thesis by(simp add:is_healthy_def RH_def)
+qed
+
+(* L9 closure-sequence-R *)
+
+lemma RH_SemiR_closure:
+  assumes "P \<in> WF_RELATION" "Q\<in> WF_RELATION" "P is RH" "Q is RH"
+  shows "`P ; Q` is RH"
+proof -
+  have "`R3(P ; Q)` = `P ; Q`"
+    by (metis Healthy_simp R3_SemiR_closure RH_is_R1 RH_is_R3 assms(1) assms(2) assms(3) assms(4))
+  hence "`R2(R3(P ; Q))` = `P ; Q`" 
+    by (metis R2_SemiR_closure RH_is_R2 assms is_healthy_def)
+  hence "`R1(R2(R3(P ; Q)))` = `P ; Q`" 
+    by (metis R1_idempotent R2_def)
+  thus ?thesis by(simp add:is_healthy_def RH_def)
+qed
+
+lemma RH_form: 
+  assumes "P \<in> WF_RELATION" "P is RH"
+  shows "P = `(\<not>ok \<and> $wait \<and> ($tr \<le> $tr\<acute>)) \<or> (ok \<and> $wait \<and> II) \<or> (\<not>$wait \<and> R2(P\<^sub>f))`"
+proof-
+  have "P = RH P" by(metis is_healthy_def assms(2))
+  thus ?thesis
+  apply(simp add:RH_def R2_R3_commute R1_R3_commute)
+  apply(simp add:R3_form_2 R1_def)
+  apply(simp add:usubst typing defined closure)
+  apply(simp add:R2_wait_false)
+  apply(simp add:R2_def R1_def)
+  apply (metis (hide_lams, no_types) R1_def R1_idempotent)
+  done
+qed
 
 subsection {* The theory of Reactive Processes *}
 
 lift_definition REACTIVE :: "'VALUE WF_THEORY" 
 is "({vs. vs \<subseteq> REL_VAR \<and> REA \<subseteq> vs}, {R1,R2,R3})"
   by (simp add:WF_THEORY_def IDEMPOTENT_OVER_def R1_idempotent R2_idempotent R3_idempotent)
-
+      
 end
